<?xml version="1.0"?>
<rdf:RDF xmlns="http://vocab.ciudadesabiertas.es/def/transporte/autobus#"
	 xml:base="http://vocab.ciudadesabiertas.es/def/transporte/autobus"
	 xmlns:dc="http://purl.org/dc/elements/1.1/"
	 xmlns:dct="http://purl.org/dc/terms/"
	 xmlns:esautob="http://vocab.ciudadesabiertas.es/def/transporte/autobus#"
	 xmlns:escjr="http://vocab.linkeddata.es/datosabiertos/def/urbanismo-infraestructuras/callejero#"
	 xmlns:esdir="http://vocab.linkeddata.es/datosabiertos/def/urbanismo-infraestructuras/direccion-postal#"
	 xmlns:estraf="http://vocab.ciudadesabiertas.es/def/transporte/trafico#"
	 xmlns:geo="http://www.w3.org/2003/01/geo/wgs84_pos#"
	 xmlns:geocore="https://datos.ign.es/def/geo_core#"
	 xmlns:geosparql="http://www.opengis.net/ont/geosparql#"
	 xmlns:owl="http://www.w3.org/2002/07/owl#"
	 xmlns:rdf="http://www.w3.org/1999/02/22-rdf-syntax-ns#"
	 xmlns:rdfs="http://www.w3.org/2000/01/rdf-schema#"
	 xmlns:schema="http://schema.org"
	 xmlns:skos="http://www.w3.org/2004/02/skos/core#"
	 xmlns:sosa="http://w3.org/ns/sosa"
	 xmlns:tmcommons="http://w3id.org/transmodel/commons#"
	 xmlns:tmjourney="http://w3id.org/transmodel/journeys#"
	 xmlns:tmkos="http://w3id.org/transmodel/kos/"
	 xmlns:tmkoscommons="http://w3id.org/transmodel/kos/commons/"
	 xmlns:tmkosjourney="http://w3id.org/transmodel/kos/journeys/"
	 xmlns:tmorg="http://w3id.org/transmodel/organisations#"
	 xmlns:vann="http://purl.org/vocab/vann/"
	 xmlns:vcard="http://www.w3.org/2006/vcard#"
	 xmlns:xml="http://www.w3.org/XML/1998/namespace"
	 xmlns:xsd="http://www.w3.org/2001/XMLSchema#">
    <owl:Ontology rdf:about="http://vocab.ciudadesabiertas.es/def/transporte/autobus">
        <owl:versionIRI rdf:resource="http://vocab.ciudadesabiertas.es/def/transporte/autobus/1.0.0"/>
        <dc:contributor xml:lang="es">María Jesús Fernández Ruiz - Ayuntamiento de Zaragoza</dc:contributor>
        <dc:contributor xml:lang="es">Honorio Enrique Crespo Díaz-Alejo - Ayuntamiento de Madrid</dc:contributor>
        <dc:contributor xml:lang="es">María Carmen Ruiz Moreno - Ayuntamiento de Madrid</dc:contributor>
	<dc:contributor xml:lang="es">María Jesús Gallego San Miguel - Ayuntamiento de Madrid</dc:contributor>
        <dc:contributor xml:lang="es">María del Mar Arribas de Andrés - Ayuntamiento de Madrid</dc:contributor>
	<dc:contributor xml:lang="es">Servicio de Innovación y Desarrollo Tecnológico - Ayuntamiento de A Coruña</dc:contributor>
	<dc:contributor xml:lang="es">Víctor Morlán Pío - Ayuntamiento de Zaragoza</dc:contributor>
        <dc:contributor xml:lang="es">Red.es</dc:contributor>
        <dc:contributor xml:lang="es">Servicio de Informática - Ayuntamiento de Santiago de Compostela</dc:contributor>
	<dc:creator rdf:datatype="http://www.w3.org/2001/XMLSchema#string">Adolfo Antón Bravo (Ontology Engineering Group - Universidad Politécnica de Madrid)</dc:creator>
        <dc:creator rdf:datatype="http://www.w3.org/2001/XMLSchema#string">Edna Ruckhaus (Ontology Engineering Group - Universidad Politécnica de Madrid)</dc:creator>
	<dc:creator rdf:datatype="http://www.w3.org/2001/XMLSchema#string">Paola Espinoza Arias (Ontology Engineering Group - Universidad Politécnica de Madrid)</dc:creator>
        <dc:creator rdf:datatype="http://www.w3.org/2001/XMLSchema#string">Oscar Corcho (Ontology Engineering Group - Universidad Politécnica de Madrid, Localidata)</dc:creator>
        <dc:identifier xml:lang="es">http://vocab.ciudadesabiertas.es/def/transporte/autobus</dc:identifier>
        <dc:rights>Creative Commons Attribution 4.0 International (CC BY 4.0)</dc:rights>
        <dc:title xml:lang="es">Vocabulario para la representación de datos sobre el transporte público urbano de autobuses.</dc:title>
        <dc:title xml:lang="en">Vocabulary for the representation of data on public transport by bus.</dc:title>
	<dc:description xml:lang="es" rdf:datatype="http://www.w3.org/2001/XMLSchema#string">Este vocabulario está siendo desarrollado en el contexto de la actuación sobre datos abiertos del proyecto "Plataforma de Gobierno Abierto, Colaborativa e Interoperable" de la "II Convocatoria de Ciudades Inteligentes" del Ministerio de Economía y Empresa lanzada a través de la Entidad Pública Empresarial Red.es adscrita a la Secretaría de estado de Avance Digital de dicho ministerio.</dc:description>
	<dc:description xml:lang="en" rdf:datatype="http://www.w3.org/2001/XMLSchema#string">This vocabulary is being developed in the context of the action on open data of the project "Platform of Open, Collaborative and Interoperable Government" of the "II Call for Intelligent Cities" of the Ministry of Economy and Enterprise launched through the Public Business Entity Red.es assigned to the Secretariat of State for Digital Progress of the Ministry.</dc:description>
	<dc:abstract xml:lang="es" rdf:datatype="http://www.w3.org/2001/XMLSchema#string">El vocabulario de Autobús trabaja con el estándar europeo TransModel (EN 12896 realizado por el CEN, Comité Europeo de Normalización) que ha sido adoptado por el reglamento europeo 2017/1926 y que sigue la directiva europea sobre servicios inteligentes de transporte (Directiva 2010/40/UE sobre ITS,Intelligent Transport System).
Desde diciembre de 2019 este reglamento ha entrado en vigor y dictamina que cualquier operador o autoridad de transporte europea debe ofrecer sus datos en formatos compatibles con Transmodel.
Esta ontología se basa en el trabajo previo realizado durante el proyecto SNAP (snap-project.eu) donde se realizó una primera versión de la ontología transmodel.
En general se han reusado los siguientes conceptos de Transmodel: Operador, Autoridad, Línea, Ruta, Puntos en una Ruta, Patrón de Viaje, Puntos en un Patrón de Viaje, Parada, Viaje asociado a un Patrón de Viaje, Horarios y Frecuencias de un Viaje y Calendario de Servicio.
Este vocabulario realiza otras relaciones: con el concepto de Incidencia que se ha desarrollado en el vocabulario de Tráfico del mismo proyecto de Ciudades Abiertas; con el vocabularios de Dirección Postal; con geosparql para la representación geográfica.
El vocabulario se ha dividido en tres grandes partes:
- Organizaciones (autoridad y operador) y sus líneas
- Rutas y puntos de las mismas, incluidas las paradas.
- Viajes y patrones de viaje
</dc:abstract>
<dc:abstract xml:lang="en" rdf:datatype="http://www.w3.org/2001/XMLSchema#string">The Bus Vocabulary works with the European standard TransModel (EN 12896 made by CEN, European Committee for Standardization) which has been adopted by the European regulation 2017/1926 and follows the European directive on intelligent transport services (Directive 2010/40/EU on ITS,Intelligent Transport System).
Since December 2019 this regulation has come into force and dictates that any European operator or transport authority must offer its data in formats compatible with Transmodel.
This ontology is based on the previous work carried out during the SNAP project (snap-project.eu) where a first version of the Transmodel ontology was developed.
In general, the following Transmodel concepts have been reused: Operator, Authority, Line, Route, Points on a Route, Trip Pattern, Points on a Trip Pattern, Stop, Trip associated to a Trip Pattern, Timetables and Frequencies of a Trip and Service Calendar.
This vocabulary makes other relations: with the concept of Incidence that has been developed in the Traffic vocabulary of the same Open Cities project; with the Postal Address vocabulary; with geosparql for the geographical representation.
The vocabulary has been divided into three main parts:
- Organizations (authority and operator) and their lines.
- Routes and points thereof, including stops.
- Journeys and travel patterns.
	</dc:abstract>
	<vann:preferredNamespacePrefix>esautob</vann:preferredNamespacePrefix>
	<vann:preferredNamespaceUri rdf:resource="http://vocab.ciudadesabiertas.es/def/transporte/autobus#"/>
	<dct:publisher xml:lang="es">Ontology Engineering Group - Universidad Politécnica de Madrid</dct:publisher>
	<dct:publisher xml:lang="en">Ontology Engineering Group - Universidad Politécnica de Madrid</dct:publisher>
        <dct:hasVersion>1.0.0</dct:hasVersion>
	<dct:created rdf:datatype="http://www.w3.org/2001/XMLSchema#dateTime">2020-05-05</dct:created>
        <dct:issued rdf:datatype="http://www.w3.org/2001/XMLSchema#dateTime">2020-05-07</dct:issued>
        <dct:license rdf:datatype="http://www.w3.org/2001/XMLSchema#string">https://creativecommons.org/licenses/by/4.0</dct:license>
        <rdfs:comment xml:lang="es">Esta versión ha sido generada dentro del contexto del proyecto Plataforma de gobierno abierto, colaborativa e interoperable en el que participan los ayuntamientos de Madrid, Zaragoza, Santiago de Compostela y A Coruña. En esta versión se han definido clases y propiedades de acuerdo a los requisitos y glosario de conceptos propuestos en las reuniones del grupo.</rdfs:comment>
	<rdfs:comment xml:lang="en">This version has been generated within the context of the project Open, collaborative and interoperable government platform in which the city councils of Madrid, Zaragoza, Santiago de Compostela and A Coruña participate. In this version, classes and properties have been defined according to the requirements and glossary of concepts proposed at the group's meetings.</rdfs:comment>
        <owl:versionInfo xml:lang="es">Versión 1.0 de la ontología de Tráfico que ha sido implementada en el contexto del proyecto Plataforma de gobierno abierto, colaborativa e interoperable en la que participan los ayuntamientos de Madrid, Zaragoza, Santiago de Compostela y A Coruña.</owl:versionInfo>
	<owl:versionInfo xml:lang="en">This is the initial version of the Traffic ontology that has been implemented in the context of the project Open, collaborative and interoperable government platform in which the city councils of Madrid, Zaragoza, Santiago de Compostela and A Coruña participate.</owl:versionInfo>
    </owl:Ontology>
    


    <!-- 
	 ///////////////////////////////////////////////////////////////////////////////////////
	 //
	 // Annotation properties
	 //
	 ///////////////////////////////////////////////////////////////////////////////////////
    -->

    <!-- http://purl.org/dc/elements/1.1/abstract -->

    <owl:AnnotationProperty rdf:about="http://purl.org/dc/elements/1.1/abstract"/>

    <!-- http://purl.org/dc/elements/1.1/contributor -->

    <owl:AnnotationProperty rdf:about="http://purl.org/dc/elements/1.1/contributor"/>

     <!-- http://purl.org/dc/elements/1.1/creator -->

    <owl:AnnotationProperty rdf:about="http://purl.org/dc/elements/1.1/creator"/>
    
    <!-- http://purl.org/dc/elements/1.1/date -->

    <owl:AnnotationProperty rdf:about="http://purl.org/dc/elements/1.1/date"/>

    <!-- http://purl.org/dc/elements/1.1/description -->

    <owl:AnnotationProperty rdf:about="http://purl.org/dc/elements/1.1/description"/>

    <!-- http://purl.org/dc/elements/1.1/identifier -->

    <owl:AnnotationProperty rdf:about="http://purl.org/dc/elements/1.1/identifier"/>

    <!-- http://purl.org/dc/elements/1.1/rights -->

    <owl:AnnotationProperty rdf:about="http://purl.org/dc/elements/1.1/rights"/>

    <!-- http://purl.org/dc/elements/1.1/title -->

    <owl:AnnotationProperty rdf:about="http://purl.org/dc/elements/1.1/title"/>

    <!-- http://purl.org/dc/terms/created -->

    <owl:AnnotationProperty rdf:about="http://purl.org/dc/terms/created"/>

    <!-- http://purl.org/dc/terms/hasVersion -->

    <owl:AnnotationProperty rdf:about="http://purl.org/dc/terms/hasVersion"/>
    
    <!-- http://purl.org/dc/terms/issued -->

    <owl:AnnotationProperty rdf:about="http://purl.org/dc/terms/issued">
        <dct:hasVersion rdf:resource="http://dublincore.org/usage/terms/history/#issued-003"/>
        <rdfs:comment xml:lang="en">Date of formal issuance (e.g., publication) of the resource.</rdfs:comment>
        <rdfs:isDefinedBy xml:lang="en">http://purl.org/dc/terms/</rdfs:isDefinedBy>
        <rdfs:label xml:lang="en">Date Issued</rdfs:label>
        <rdfs:subPropertyOf rdf:resource="http://purl.org/dc/elements/1.1/date"/>
    </owl:AnnotationProperty>

    <!-- http://purl.org/dc/terms/license -->

    <owl:AnnotationProperty rdf:about="http://purl.org/dc/terms/license"/>

    <!-- http://purl.org/dc/terms/publisher -->

    <owl:AnnotationProperty rdf:about="http://purl.org/dc/terms/publisher"/>

    <!-- http://www.w3.org/2004/02/skos/core#definition -->

    <owl:AnnotationProperty rdf:about="http://www.w3.org/2004/02/skos/core#definition"/>

    <!-- http://purl.org/vocab/vann/preferredNamespacePrefix -->

    <owl:AnnotationProperty rdf:about="http://purl.org/vocab/vann/preferredNamespacePrefix"/>

    <!-- http://purl.org/vocab/vann/preferredNamespaceUri -->

    <owl:AnnotationProperty rdf:about="http://purl.org/vocab/vann/preferredNamespaceUri"/>



    <!-- 
	 ///////////////////////////////////////////////////////////////////////////////////////
	 //
	 // Datatypes
	 //
	 ///////////////////////////////////////////////////////////////////////////////////////
    -->

    


    <!-- http://www.w3.org/2001/XMLSchema#date -->

    <rdfs:Datatype rdf:about="http://www.w3.org/2001/XMLSchema#date"/>
    


    <!-- 
	 ///////////////////////////////////////////////////////////////////////////////////////
	 //
	 // Object Properties
	 //
	 ///////////////////////////////////////////////////////////////////////////////////////
    -->

    
    <!-- http://vocab.ciudadesabiertas.es/def/transporte/autobus#afectadaPorIncidencia -->

    <owl:ObjectProperty rdf:about="http://vocab.ciudadesabiertas.es/def/transporte/autobus#afectadaPorIncidencia">
      <rdfs:subPropertyOf rdf:resource="http://www.w3.org/2002/07/owl#topObjectProperty"/>
      <rdfs:domain>
	<owl:Class>
	  <owl:unionOf rdf:parseType="Collection">
	    <rdf:Description rdf:about="http://vocab.ciudadesabiertas.es/def/transporte/autobus#Linea"/>
	    <rdf:Description rdf:about="http://w3id.org/transmodel/journeys#JourneyPattern"/>
	  </owl:unionOf>
	</owl:Class>
      </rdfs:domain>
      <rdfs:range rdf:resource="http://vocab.ciudadesabiertas.es/def/transporte/trafico#Incidencia"/>
      <rdfs:comment xml:lang="es">Relación de una línea que está afectada por una incidencia.</rdfs:comment>
      <rdfs:comment xml:lang="en">Relationship of a line affected by an incidence.</rdfs:comment>
      <rdfs:isDefinedBy rdf:resource="http://vocab.ciudadesabiertas.es/def/transporte/autobus"/>
      <rdfs:label xml:lang="es">línea afectada por incidencia</rdfs:label>
      <rdfs:label xml:lang="en">line affected by an incidence</rdfs:label>
    </owl:ObjectProperty>

    <!-- http://vocab.ciudadesabiertas.es/def/transporte/autobus#cabeceraLinea -->

    <owl:ObjectProperty rdf:about="http://vocab.ciudadesabiertas.es/def/transporte/autobus#cabeceraLinea">
      <rdfs:subPropertyOf rdf:resource="http://www.w3.org/2002/07/owl#topObjectProperty"/>
        <rdfs:domain
	    rdf:resource="http://vocab.ciudadesabiertas.es/def/transporte/autobus#Linea"/>
        <rdfs:range rdf:resource="http://vocab.ciudadesabiertas.es/def/transporte/autobus#Parada"/>
        <rdfs:comment xml:lang="es">Indica cuál es la parada de cabecera de la línea.</rdfs:comment>
        <rdfs:comment xml:lang="en">Points out which stop point is the heading of the line.</rdfs:comment>
        <rdfs:isDefinedBy rdf:resource="http://vocab.ciudadesabiertas.es/def/transporte/autobus"/>
        <rdfs:label xml:lang="es">Cabecera de Línea</rdfs:label>
        <rdfs:label xml:lang="en">Line Head Stop Point</rdfs:label>
    </owl:ObjectProperty>

    <!-- http://vocab.ciudadesabiertas.es/def/transporte/autobus#finalLinea -->

    <owl:ObjectProperty rdf:about="http://vocab.ciudadesabiertas.es/def/transporte/autobus#finalLinea">
      <rdfs:subPropertyOf rdf:resource="http://www.w3.org/2002/07/owl#topObjectProperty"/>
        <rdfs:domain
	    rdf:resource="http://vocab.ciudadesabiertas.es/def/transporte/autobus#Linea"/>
        <rdfs:range rdf:resource="http://vocab.ciudadesabiertas.es/def/transporte/autobus#Parada"/>
        <rdfs:comment xml:lang="es">Indica cuál es la parada de final de la línea.</rdfs:comment>
        <rdfs:comment xml:lang="en">Points out which stop point is the end of the line.</rdfs:comment>
        <rdfs:isDefinedBy rdf:resource="http://vocab.ciudadesabiertas.es/def/transporte/autobus"/>
        <rdfs:label xml:lang="es">Final de Línea</rdfs:label>
        <rdfs:label xml:lang="en">Line End Stop Point</rdfs:label>
    </owl:ObjectProperty>

    <!-- http://vocab.ciudadesabiertas.es/def/transporte/autobus#ubicacion -->

    <owl:ObjectProperty rdf:about="http://vocab.ciudadesabiertas.es/def/transporte/autobus#ubicacion">
      <rdfs:subPropertyOf rdf:resource="http://www.w3.org/2002/07/owl#topObjectProperty"/>
      <rdfs:domain rdfs:resource="http://vocab.ciudadesabiertas.es/def/transporte/autobus#Parada"/>
      <rdfs:range rdf:resource="http://www.opengis.net/ont/geosparql#Point"/>
      <rdfs:comment xml:lang="es">Ubicación de la Parada según coordenadas WGS84</rdfs:comment>
      <rdfs:comment xml:lang="en">Stop Point Location according to WGS84</rdfs:comment>
      <rdfs:label xml:lang="es">Ubicación Parada</rdfs:label>
      <rdfs:label xml:lang="en">Stop Point Location</rdfs:label>
    </owl:ObjectProperty>
    
    <!-- http://www.w3.org/2004/02/skos/core#inScheme -->
    
    <owl:ObjectProperty rdf:about="http://www.w3.org/2004/02/skos/core#inScheme">
      <rdfs:subPropertyOf rdf:resource="http://www.w3.org/2002/07/owl#topObjectProperty"/>
	<rdfs:range rdf:resource="http://www.w3.org/2004/02/skos/core#ConceptScheme"/>
	<rdfs:isDefinedBy rdf:resource="http://www.w3.org/2004/02/skos/core"/>
	<rdfs:label xml:lang="en">It is in Scheme</rdfs:label>
	<rdfs:label xml:lang="es">En taxonomía</rdfs:label>
	<skos:definition xml:lang="en">Relates a resource (for example a concept) to a concept scheme in which it is included.</skos:definition>
	<skos:definition xml:lang="es">Relaciona un recurso, como por ejemplo un concepto, con un esquema de conceptos o taxonomía en el que se incluye.</skos:definition>
    </owl:ObjectProperty>

    <!-- http://w3id.org/transmodel/journeys#composedOf -->

    <owl:ObjectProperty rdf:about="http://w3id.org/transmodel/journeys#composedOf">
        <rdfs:domain rdf:resource="http://w3id.org/transmodel/journeys#VehicleJourney"/>
        <rdfs:range rdf:resource="http://w3id.org/transmodel/journeys#HeadwayJourneyGroup"/>
        <rdfs:comment xml:lang="en">This property relates a Vehicle Journey with the Headway Journey Group which sets the first and last departure time.</rdfs:comment>
	<rdfs:comment xml:lang="es">Un Viaje de Vehículo compuesto de indicaciones de viaje en cabecera de línea donde se indican las salidas del primero y último viaje.</rdfs:comment>
        <rdfs:label xml:lang="en">composed of</rdfs:label>
	<rdfs:label xml:lang="es">Se compone de</rdfs:label>
    </owl:ObjectProperty>

    <!-- http://w3id.org/transmodel/journeys#definedBy -->

    <owl:ObjectProperty rdf:about="http://w3id.org/transmodel/journeys#definedBy">
        <rdfs:domain rdf:resource="http://w3id.org/transmodel/journeys#ServiceCalendar"/>
        <rdfs:range rdf:resource="http://w3id.org/transmodel/journeys#DayTypeAssignment"/>
        <rdfs:comment xml:lang="en">This property sets the relationship between Service Calendar and Day Type Assignment</rdfs:comment>
	<rdfs:comment xml:lang="es">Establece la relación entre un Calendario de Servicio y la Asignación de Día Tipo.</rdfs:comment>
        <rdfs:label xml:lang="en">defined By</rdfs:label>
	<rdfs:label xml:lang="es">definición por</rdfs:label>
    </owl:ObjectProperty>

   
 <!-- http://w3id.org/transmodel/journeys#determinedBy -->

    <owl:ObjectProperty rdf:about="http://w3id.org/transmodel/journeys#determinedBy">
        <rdfs:domain rdf:resource="http://w3id.org/transmodel/journeys#HeadwayJourneyGroup"/>
        <rdfs:range rdf:resource="http://w3id.org/transmodel/journeys#HeadwayInterval"/>
	<rdfs:comment xml:lang="en">A Headway Journey Group determined by a Headway Interval</rdfs:comment>
	<rdfs:comment xml:lang="es">Un grupo de viajes de cabecera de línea con un intervalo desde cabecera de línea</rdfs:comment>
	<rdfs:label xml:lang="en">determined By</rdfs:label>
	<rdfs:label xml:lang="es">determinado por</rdfs:label>
    </owl:ObjectProperty>

    <!-- http://w3id.org/transmodel/journeys#directionType -->

    <owl:ObjectProperty rdf:about="http://w3id.org/transmodel/journeys#directionType">
        <rdfs:subPropertyOf rdf:resource="http://www.w3.org/2002/07/owl#topObjectProperty"/>
        <rdfs:domain rdf:resource="http://w3id.org/transmodel/journeys#Route"/>
        <rdfs:range>
            <owl:Class>
                <owl:intersectionOf rdf:parseType="Collection">
                    <rdf:Description rdf:about="http://www.w3.org/2004/02/skos/core#Concept"/>
                    <owl:Restriction>
                        <owl:onProperty rdf:resource="http://www.w3.org/2004/02/skos/core#inScheme"/>
                        <owl:hasValue rdf:resource="http://w3id.org/transmodel/kos/journeys/direction-type"/>
                    </owl:Restriction>
                </owl:intersectionOf>
            </owl:Class>
        </rdfs:range>
        <rdfs:comment xml:lang="en">This property allows describing the type of direction for a Route</rdfs:comment>
	<rdfs:comment xml:lang="es">Esta propiedad permite describir el tipo de dirección para una Ruta.</rdfs:comment>
        <rdfs:label xml:lang="en">Direction Type</rdfs:label>
	<rdfs:label xml:lang="es">Tipo de Dirección</rdfs:label>
    </owl:ObjectProperty>

    <!-- http://w3id.org/transmodel/journeys#functionalCentroidFor -->

    <owl:ObjectProperty rdf:about="http://w3id.org/transmodel/journeys#aFunctionalCentroidFor">
        <rdfs:subPropertyOf rdf:resource="http://www.w3.org/2002/07/owl#topObjectProperty"/>
        <rdfs:domain rdf:resource="http://w3id.org/transmodel/journeys#Point"/>
        <rdfs:range rdf:resource="http://w3id.org/transmodel/journeys#Zone"/>
        <rdfs:comment xml:lang="en">This property allows connecting a Point with a Zone.</rdfs:comment>
	<rdfs:comment xml:lang="es">Esta propiedad permite la conexión de un Punto con una Zona.</rdfs:comment>
        <rdfs:label xml:lang="en">aFunctionalCentroidFor</rdfs:label>
	<rdfs:label xml:lang="es">Un centroide funcional para</rdfs:label>
    </owl:ObjectProperty>

     <!-- http://w3id.org/transmodel/journeys#includedIn -->

 <owl:ObjectProperty rdf:about="http://w3id.org/transmodel/journeys#includedIn">
   <rdfs:subPropertyOf rdf:resource="http://www.w3.org/2002/07/owl#topObjectProperty"/>
   <rdfs:domain rdf:resource="http://w3id.org/transmodel/journeys#ScheduledStopPoint"/>
   <rdfs:range rdf:resource="http://w3id.org/transmodel/journeys#StopArea"/>
      <rdfs:comment xml:lang="en">A Scheduled Stop Point can be next to other Stop Points so they can be included in a Stop Area.</rdfs:comment>
      <rdfs:comment xml:lang="es">Una Parada Programada (Scheduled Stop Point) puede estar próxima a otras por lo que pueden todas ellas formas parte de una zona de Paradas.</rdfs:comment>
      <rdfs:label xml:lang="en">Included In</rdfs:label>
      <rdfs:label xml:lang="es">Incluida en</rdfs:label>
    </owl:ObjectProperty>

    <!-- http://w3id.org/transmodel/journeys#madeUpOf -->
    
    <owl:ObjectProperty rdf:about="http://w3id.org/transmodel/journeys#madeUpOf">
      <rdfs:subPropertyOf rdf:resource="http://www.w3.org/2002/07/owl#topObjectProperty"/>
        <rdfs:comment xml:lang="en">Relationship between entities made up of other entities</rdfs:comment>
	<rdfs:comment xml:lang="es">Relación entre entidades hechas de otras entidades.</rdfs:comment>
        <rdfs:label xml:lang="en">made Up Of</rdfs:label>
	<rdfs:label xml:lang="es">compuesto por</rdfs:label>
    </owl:ObjectProperty>

    <!-- http://w3id.org/transmodel/journeys#madeUsing -->

    <owl:ObjectProperty rdf:about="http://w3id.org/transmodel/journeys#madeUsing">
      <rdfs:subPropertyOf rdf:resource="http://www.w3.org/2002/07/owl#topObjectProperty"/>
      <rdfs:domain rdf:resource="http://w3id.org/transmodel/journeys#LinkSequence"/>
      <rdfs:range rdf:resource="http://w3id.org/transmodel/journeys#PointInLinkSequence"/>
        <rdfs:comment xml:lang="en">This property connects some classes to other classes that makes its behaviour possible</rdfs:comment>
	<rdfs:comment xml:lang="es">Esta propiedad conecta algunas clases con otras que hacen posible su funcionamiento.</rdfs:comment>
        <rdfs:label xml:lang="en">made Using</rdfs:label>
	<rdfs:label xml:lang="es">se hace con</rdfs:label>
    </owl:ObjectProperty>

    <!-- http://w3id.org/transmodel/journeys#on -->

    <owl:ObjectProperty rdf:about="http://w3id.org/transmodel/journeys#on">
      <rdfs:subPropertyOf rdf:resource="http://www.w3.org/2002/07/owl#topObjectProperty"/>
      <rdfs:domain rdf:resource="http://w3id.org/transmodel/journeys#JourneyPattern"/>
      <rdfs:range rdf:resource="http://w3id.org/transmodel/journeys#Route"/>
        <rdfs:comment xml:lang="en">This property connects the JourneyPattern with the Route where it works</rdfs:comment>
	<rdfs:comment xml:lang="es">Esta propiedad conecta el patrón de viaje con la ruta en la que trabaja.</rdfs:comment>
        <rdfs:label xml:lang="en">on</rdfs:label>
	<rdfs:label xml:lang="es">en</rdfs:label>
    </owl:ObjectProperty>

        <!-- http://w3id.org/transmodel/journeys#prescribing -->

    <owl:ObjectProperty rdf:about="http://w3id.org/transmodel/journeys#prescribing">
      <rdfs:subPropertyOf rdf:resource="http://www.w3.org/2002/07/owl#topObjectProperty"/>
      <rdfs:domain rdf:resource="http://w3id.org/transmodel/journeys#JourneyPattern"/>
      <rdfs:range rdf:resource="http://w3id.org/transmodel/journeys#DestinationDisplay"/>
      <rdfs:comment xml:lang="en">A Journey Pattern is prescribing a Destination Display</rdfs:comment>
      <rdfs:comment xml:lang="en">Un patrón de viaje que anuncia su destino de alguna forma</rdfs:comment>
      <rdfs:label xml:lang="en">Prescribing</rdfs:label>
      <rdfs:label xml:lang="es">Prescribe</rdfs:label>
    </owl:ObjectProperty>

        <!-- http://w3id.org/transmodel/journeys#presentedBy -->

    <owl:ObjectProperty rdf:about="http://w3id.org/transmodel/journeys#presentedBy">
        <rdfs:domain rdf:resource="http://w3id.org/transmodel/journeys#Line"/>
        <rdfs:range rdf:resource="http://w3id.org/transmodel/commons#Presentation"/>
        <rdfs:comment xml:lang="en">This property is used to connect a Line with its corresponding Presentation</rdfs:comment>
	<rdfs:comment xml:lang="es">Esta propiedad se utiliza para conectar una línea con su correspondiente forma de presentarse en Presentation, donde por ejemplo se indica eel color de línea o el color del texto.</rdfs:comment>
        <rdfs:label xml:lang="en">presented by</rdfs:label>
	<rdfs:label xml:lang="es">Anunciada por</rdfs:label>
    </owl:ObjectProperty>

    <!-- http://w3id.org/transmodel/journeys#specifying -->

    <owl:ObjectProperty rdf:about="http://w3id.org/transmodel/journeys#specifying">
        <rdfs:subPropertyOf rdf:resource="http://www.w3.org/2002/07/owl#topObjectProperty"/>
        <rdfs:domain rdf:resource="http://w3id.org/transmodel/journeys#DayTypeAssignment"/>
        <rdfs:range rdf:resource="http://w3id.org/transmodel/journeys#DayType"/>
        <rdfs:comment xml:lang="en">The assignment of operational characteristics, expressed by DayType, to a particular OperatingDay within a ServiceCalendar</rdfs:comment>
	<rdfs:comment xml:lang="en">La asignación de características operativas expresadas en Día Tipo a un Día Operativo particular dentro de un Calendario de Servicio.</rdfs:comment>
        <rdfs:label xml:lang="en">specifying</rdfs:label>
	<rdfs:label xml:lang="es">especifica</rdfs:label>
    </owl:ObjectProperty>

    <!-- http://w3id.org/transmodel/journeys#stopUse -->

    <owl:ObjectProperty rdf:about="http://w3id.org/transmodel/journeys#stopUse">
        <rdfs:subPropertyOf rdf:resource="http://www.w3.org/2002/07/owl#topObjectProperty"/>
        <rdfs:domain rdf:resource="http://w3id.org/transmodel/journeys#StopPointInJourneyPattern"/>
        <rdfs:range>
            <owl:Class>
                <owl:intersectionOf rdf:parseType="Collection">
                    <rdf:Description rdf:about="http://www.w3.org/2004/02/skos/core#Concept"/>
                    <owl:Restriction>
                        <owl:onProperty rdf:resource="http://www.w3.org/2004/02/skos/core#inScheme"/>
                        <owl:hasValue rdf:resource="http://w3id.org/transmodel/kos/journeys/stop-use-type"/>
                    </owl:Restriction>
                </owl:intersectionOf>
            </owl:Class>
        </rdfs:range>
        <rdfs:comment xml:lang="en">This property allows describing the type of use of a stop (e.g., access, interchange only, pass through)</rdfs:comment>
	<rdfs:comment xml:lang="es">Permite la descripción del tipo de uso de una parada: acceso, intercambio, de paso, etc.</rdfs:comment>
	<rdfs:label xml:lang="es">función de la parada</rdfs:label>
        <rdfs:label xml:lang="en">stop Use</rdfs:label>
    </owl:ObjectProperty>

    <!-- http://w3id.org/transmodel/journeys#timedFrom -->

    <owl:ObjectProperty rdf:about="http://w3id.org/transmodel/journeys#timedFrom">
      <rdfs:subPropertyOf rdf:resource="http://www.w3.org/2002/07/owl#topObjectProperty"/>
      <rdfs:domain rdf:resource="http://w3id.org/transmodel/journeys#VehicleJourney"/>
      <rdfs:range rdf:resource="http://w3id.org/transmodel/journeys#TimingPointInJourneyPattern"/>
      <rdfs:comment xml:lang="en">The relationship between a sort of Journey and a sort of Timing Point</rdfs:comment>
      <rdfs:comment xml:lang="es">Indica el punto del Viaje del Vehículo donde se toman los tiempos.</rdfs:comment>
      <rdfs:comment xml:lang="es">ToDo: Valorar si se trata de una medición SOSA para próxima versión</rdfs:comment>
      <rdfs:label xml:lang="en">timedFrom</rdfs:label>
      <rdfs:label xml:lang="es">toma de tiempo</rdfs:label>
    </owl:ObjectProperty>

    <!-- http://w3id.org/transmodel/journeys#viewedAs -->

    <owl:ObjectProperty rdf:about="http://w3id.org/transmodel/journeys#viewedAs">
        <rdfs:subPropertyOf rdf:resource="http://www.w3.org/2002/07/owl#topObjectProperty"/>
        <rdfs:domain rdf:resource="http://w3id.org/transmodel/journeys#PointInLinkSequence"/>
        <rdfs:range rdf:resource="http://w3id.org/transmodel/journeys#Point"/>
        <rdfs:comment xml:lang="en">This property allows connecting a Point in Link Sequence with the corresponding Point</rdfs:comment>
	<rdfs:comment xml:lang="es">Esta propiedad relaciona un Punto en una secuencia con un Punto ya que es una forma de verlo.</rdfs:comment>
        <rdfs:label xml:lang="en">viewed As</rdfs:label>
	<rdfs:label xml:lang="es">Se ve como</rdfs:label>
    </owl:ObjectProperty>


    <!-- http://w3id.org/transmodel/journeys#workedOn -->

    <owl:ObjectProperty rdf:about="http://w3id.org/transmodel/journeys#workedOn">
      <rdfs:subPropertyOf rdf:resource="http://www.w3.org/2002/07/owl#topObjectProperty"/>
        <rdfs:domain rdf:resource="http://w3id.org/transmodel/journeys#VehicleJourney"/>
        <rdfs:range rdf:resource="http://w3id.org/transmodel/journeys#DayType"/>
        <rdfs:comment xml:lang="en">This property sets the relationship between Vehicle Journey and Day Type.</rdfs:comment>
	<rdfs:comment xml:lang="es">Relación entre el Viaje de un Vehículo y el Día Tipo.</rdfs:comment>
	<rdfs:label xml:lang="en">worked On</rdfs:label>
	<rdfs:label xml:lang="es">Opera en</rdfs:label>
    </owl:ObjectProperty>
    
    <!-- http://w3id.org/transmodel/organisations#characterisedBy -->

    <owl:ObjectProperty rdf:about="http://w3id.org/transmodel/organisations#characterisedBy">
      <rdfs:subPropertyOf rdf:resource="http://www.w3.org/2002/07/owl#topObjectProperty"/>
      <rdfs:subPropertyOf rdf:resource="http://schema.org/contactPoint"/>
        <rdfs:domain rdf:resource="http://w3id.org/transmodel/organisations#Organisation"/>
        <rdfs:range rdf:resource="http://w3id.org/transmodel/organisations#ContactDetails"/>
        <rdfs:comment xml:lang="en">This property relates an Organisation with its corresponding Contact Details. It is a subproperty of schema:contactPoint, which relates anything to a ContactPoint</rdfs:comment>
	<rdfs:comment xml:lang="es">Una organización tiene información de contacto. Es una subpropiedad de schema:contacPoint que aporta información de contacto para una persona u organización a través de la clase schema:ContactPoint.</rdfs:comment>
        <rdfs:label xml:lang="en">characterised by</rdfs:label>
	<rdfs:label xml:lang="es">caracterizada por</rdfs:label>
    </owl:ObjectProperty>

    <!-- http://w3id.org/transmodel/organisations#operating -->

    <owl:ObjectProperty rdf:about="http://w3id.org/transmodel/organisations#operating">
      <rdfs:subPropertyOf rdf:resource="http://www.w3.org/2002/07/owl#topObjectProperty"/>
      <rdfs:domain rdf:resource="http://w3id.org/transmodel/organisations#Operator"/>
      <rdfs:range rdf:resource="http://w3id.org/transmodel/journeys#Line"/>
      <rdfs:comment xml:lang="en">This property points out what Lines are operated by what Operator</rdfs:comment>
      <rdfs:comment xml:lang="es">Esta propiedad señala qué Líneas están operadas por qué Operador.</rdfs:comment>
      <rdfs:label xml:lang="en">operating</rdfs:label>
      <rdfs:label xml:lang="es">operando</rdfs:label>
    </owl:ObjectProperty>

    <!-- http://w3id.org/transmodel/organisations#servingPTFor -->

    <owl:ObjectProperty rdf:about="http://w3id.org/transmodel/organisations#servingPTFor">
      <rdfs:subPropertyOf rdf:resource="http://www.w3.org/2002/07/owl#topObjectProperty"/>
      <rdfs:domain rdf:resource="http://w3id.org/transmodel/organisations#Operator"/>
      <rdfs:range rdf:resource="http://w3id.org/transmodel/organisations#Authority"/>
      <rdfs:comment xml:lang="en">This property points out for with Authority is working for the Operator</rdfs:comment>
      <rdfs:comment xml:lang="es">Esta propiedad indica para qué Autoridad está trabajando la entidad operadora.</rdfs:comment>
      <rdfs:label xml:lang="en">Serving Public Transport For</rdfs:label>
      <rdfs:label xml:lang="es">Sirve el Transporte Público para</rdfs:label>
    </owl:ObjectProperty>

    <!-- http://schema.org/contactPoint -->

    <owl:ObjectProperty rdf:about="http://schema.org/contactPoint">
      <rdfs:subPropertyOf rdf:resource="http://www.w3.org/2002/07/owl#topObjectProperty"/>
      <rdfs:domain rdf:resource="http://w3id.org/transmodel/organisations#Organisation"/>
      <rdfs:range rdf:resource="http://schema.org/ContactPoint"/>
      <rdfs:comment xml:lang="en">A contact point for a person or organization.</rdfs:comment>
      <rdfs:comment xml:lang="es">Un Punto de Información de Contacto para una persona u organización.</rdfs:comment>
      <rdfs:label xml:lang="en">Contact Point</rdfs:label>
      <rdfs:label xml:lang="es">Punto de Información</rdfs:label>
    </owl:ObjectProperty>

    <!-- http://schema.org/address -->

    <owl:ObjectProperty rdf:about="http://schema.org/address">
      <rdfs:subPropertyOf rdf:resource="http://www.w3.org/2002/07/owl#topObjectProperty"/>
      <rdfs:domain rdf:resource="http://vocab.ciudadesabiertas.es/def/transporte/autobus#Parada"/>
      <rdfs:range rdf:resource="http://vocab.linkeddata.es/datosabiertos/def/urbanismo-infraestructuras/direccion-postal#DireccionPostal"/>
      <rdfs:comment xml:lang="en">The address of a Stop Point</rdfs:comment>
      <rdfs:comment xml:lang="es">La dirección de una Parada.</rdfs:comment>
      <rdfs:label xml:lang="en">Has Address</rdfs:label>
      <rdfs:label xml:lang="es">Dirección</rdfs:label>
    </owl:ObjectProperty>

        <!-- http://www.w3.org/ns/sosa/hasFeatureOfInterest -->

	<owl:ObjectProperty rdf:about="http://www.w3.org/ns/sosa/hasFeatureOfInterest">
	  <rdfs:subPropertyOf rdf:resource="http://www.w3.org/2002/07/owl#topObjectProperty"/>
	  <rdfs:domain rdf:resource="http://vocab.ciudadesabiertas.es/def/transporte/autobus#RealTimePassingTime"/>
	  <rdfs:range rdf:resource="http://w3id.org/transmodel/journeys#PointInLinkSequence"/>
	  <rdfs:comment xml:lang="en">The Observation esautob:RealTimePassingTime has a feature of Interest which is tmjourney:PointInLinkSequece</rdfs:comment>
	  <rdfs:comment xml:lang="es">La observación esautob:RealTimePassingTime aparece en tmjourney:PointInLinkSequence.</rdfs:comment>
	  <rdfs:label xml:lang="en">has Feature Of Interest</rdfs:label>
	  <rdfs:label xml:lang="es">Aparece en</rdfs:label>
	</owl:ObjectProperty>
	
    


    <!-- http://www.w3.org/ns/sosa/madeBySensor -->

    <owl:ObjectProperty rdf:about="http://www.w3.org/ns/sosa/madeBySensor"/>
    


    <!-- http://www.w3.org/ns/sosa/observedProperty -->

    <owl:ObjectProperty rdf:about="http://www.w3.org/ns/sosa/observedProperty"/>
       


    <!-- http://www.w3.org/ns/sosa/observes -->

    <owl:ObjectProperty rdf:about="http://www.w3.org/ns/sosa/observes"/>




    <!-- 
	 ///////////////////////////////////////////////////////////////////////////////////////
	 //
	 // Data properties
	 //
	 ///////////////////////////////////////////////////////////////////////////////////////
    -->
    <!-- http://purl.org/dc/terms/created -->

    <owl:DatatypeProperty rdf:about="http://purl.org/dc/terms/created">
        <rdfs:domain rdf:resource="http://purl.org/dc/terms/creator"/>
        <rdfs:comment xml:lang="en">Date of creation of the resource.</rdfs:comment>
        <rdfs:comment xml:lang="es">Fecha de creación del recurso.</rdfs:comment>
        <rdfs:isDefinedBy rdf:resource="http://purl.org/dc/terms/"/>
        <rdfs:label xml:lang="es">Creado</rdfs:label>
        <rdfs:label xml:lang="en">Created</rdfs:label>
    </owl:DatatypeProperty>

    
    <!-- http://purl.org/dc/terms/description -->

    <owl:DatatypeProperty rdf:about="http://purl.org/dc/terms/description">
        <rdfs:domain>
            <owl:Class>
                <owl:unionOf rdf:parseType="Collection">
                  <rdf:Description rdf:about="http://vocab.ciudadesabiertas.es/def/transporte/autobus#Parada"/>
		  <rdf:Description rdf:about="http://w3id.org/transmodel/journeys#DayType"/>
                  <rdf:Description rdf:about="http://w3id.org/transmodel/journeys#DayTypeAssignment"/>
		  <rdf:Description rdf:about="http://w3id.org/transmodel/journeys#Route"/>
                  <rdf:Description rdf:about="http://w3id.org/transmodel/journeys#ServiceCalendar"/>
		  <rdf:Description rdf:about="http://w3id.org/transmodel/commons#Zone"/>
                </owl:unionOf>
            </owl:Class>
        </rdfs:domain>
	<rdfs:range rdf:resource="http://www.w3.org/2001/XMLSchema#string"/>
        <rdfs:comment xml:lang="en">A description of the resource within a given context.</rdfs:comment>
        <rdfs:comment xml:lang="es">Una descripción del recurso dentro de un contexto dado.</rdfs:comment>
        <rdfs:isDefinedBy rdf:resource="http://purl.org/dc/terms/"/>
        <rdfs:label xml:lang="es">Descripción</rdfs:label>
        <rdfs:label xml:lang="en">Description</rdfs:label>
    </owl:DatatypeProperty>


    <!-- http://purl.org/dc/terms/identifier -->

    <owl:DatatypeProperty rdf:about="http://purl.org/dc/terms/identifier">
        <rdfs:domain>
            <owl:Class>
              <owl:unionOf rdf:parseType="Collection">
		<rdf:Description rdf:about="http://vocab.ciudadesabiertas.es/def/transporte/autobus#Parada"/>
		<rdf:Description rdf:about="http://w3id.org/transmodel/journeys#DayType"/>
		<rdf:Description rdf:about="http://w3id.org/transmodel/journeys#DayTypeAssignment"/>
		<rdf:Description rdf:about="http://w3id.org/transmodel/journeys#HeadwayInterval"/>
		<rdf:Description rdf:about="http://w3id.org/transmodel/journeys#LinkSequence"/>
		<rdf:Description rdf:about="http://w3id.org/transmodel/journeys#PointInLinkSequence"/>
		<rdf:Description rdf:about="http://w3id.org/transmodel/journeys#StopArea"/>
		<rdf:Description rdf:about="http://w3id.org/transmodel/journeys#VehicleJourney"/>
		<rdf:Description rdf:about="http://w3id.org/transmodel/commons#Zone"/>
                </owl:unionOf>
            </owl:Class>
        </rdfs:domain>
	<rdfs:range rdf:resource="http://www.w3.org/2001/XMLSchema#string"/>
        <rdfs:comment xml:lang="en">An unambiguous reference to the resource within a given context.</rdfs:comment>
        <rdfs:comment xml:lang="es">Referencia inequívoca al recurso dentro de un contexto dado.</rdfs:comment>
        <rdfs:isDefinedBy rdf:resource="http://purl.org/dc/terms/"/>
        <rdfs:label xml:lang="es">Identificador</rdfs:label>
        <rdfs:label xml:lang="en">Identifier</rdfs:label>
    </owl:DatatypeProperty>

    <!-- http://www.w3.org/2003/01/geo/wgs84_pos#lat -->

    <owl:DatatypeProperty rdf:about=="http://www.w3.org/2003/01/geo/wgs84_pos#lat">
      <rdfs:domain rdf:resource="http://www.opengis.net/ont/sf#Point"/>
      <rdfs:range rdf:resource="http://www.w3.org/2001/XMLSchema#float"/>
      <rdfs:comment xml:lang="es">Latitud en WGS84</rdfs:comment>
      <rdfs:comment xml:lang="en">Latitude in WGS84</rdfs:comment>
      <rdfs:label>latitude</rdfs:label>
    </owl:DatatypeProperty>

    <!-- http://www.w3.org/2003/01/geo/wgs84_pos#long -->

    <owl:DatatypeProperty rdf:about=="http://www.w3.org/2003/01/geo/wgs84_pos#long">
      <rdfs:domain rdf:resource="http://www.opengis.net/ont/sf#Point"/>
      <rdfs:range rdf:resource="http://www.w3.org/2001/XMLSchema#float"/>
      <rdfs:comment xml:lang="es">Longitud en WGS84</rdfs:comment>
      <rdfs:comment xml:lang="en">Longitude in WGS84</rdfs:comment>
      <rdfs:label>longitude</rdfs:label>
    </owl:DatatypeProperty>

    <!-- https://datos.ign.es/def/geo_core#xETRS89 -->

    <owl:DatatypeProperty rdf:about="https://datos.ign.es/def/geo_core#xETRS89">
      <rdfs:domain rdf:resource="http://www.opengis.net/ont/sf#Point"/>
      <rdfs:range rdf:resource="http://www.w3.org/2001/XMLSchema#float"/>
      <dc:source xml:lang="es">Catálogo de Objetos Geográficos BTN100.</dc:source>
      <rdfs:comment xml:lang="es">Coordenada X en metros (ETRS89)</rdfs:comment>
      <rdfs:comment xml:lang="en">X-Coordinate in meters (ETRS89)</rdfs:comment>
      <rdfs:label>xETRS89</rdfs:label>
    </owl:DatatypeProperty>

    <!-- https://datos.ign.es/def/geo_core#yETRS89 -->

    <owl:DatatypeProperty rdf:about="https://datos.ign.es/def/geo_core#yETRS89">
      <rdfs:domain rdf:resource="http://www.opengis.net/ont/sf#Point"/>
      <rdfs:range rdf:resource="http://www.w3.org/2001/XMLSchema#float"/>
      <dc:source xml:lang="es">Catálogo de Objetos Geográficos BTN100.</dc:source>
      <rdfs:comment xml:lang="es">Coordenada Y en metros (ETRS89)</rdfs:comment>
      <rdfs:comment xml:lang="en">Y-Coordinate in meters (ETRS89)</rdfs:comment>
      <rdfs:label>yETRS89</rdfs:label>
    </owl:DatatypeProperty>

    <!-- http://schema.org/alternateName -->
    
    <owl:DatatypeProperty rdf:about="http://schema.org/alternateName">
        <rdfs:domain rdf:resource="http://schema.org/ContactPoint"/>
        <rdfs:range rdf:resource="http://www.w3.org/2001/XMLSchema#string"/>
        <rdfs:comment xml:lang="es">Nombre alternativo, popular o por el que se conoce a algo.</rdfs:comment>
        <rdfs:comment xml:lang="en">Alternate name, alias or popular name of some Thing.</rdfs:comment>
        <rdfs:isDefinedBy rdf:resource="http://schema.org/"/>
        <rdfs:label xml:lang="es">Alternate Name</rdfs:label>
        <rdfs:label xml:lang="en">Nombre alternativo</rdfs:label>
    </owl:DatatypeProperty>

    <!-- http://schema.org/datePosted -->

    <owl:DatatypeProperty rdf:about="http://schema.org/datePosted">
        <rdfs:domain rdf:resource="http://vocab.ciudadesabiertas.es/def/transporte/trafico#Incidencia"/>
        <rdfs:range rdf:resource="http://www.w3.org/2001/XMLSchema#dateTime"/>
        <rdfs:comment xml:lang="es">La fecha y hora de publicación de una incidencia (en formato fecha ISO 8601)</rdfs:comment>
        <rdfs:comment xml:lang="en">The end date and time of the incidence (in ISO 8601 date format).</rdfs:comment>
        <rdfs:isDefinedBy rdf:resource="http://schema.org/"/>
        <rdfs:label xml:lang="es">fecha de publicación de incidencia</rdfs:label>
        <rdfs:label xml:lang="en">posted incidence date</rdfs:label>
    </owl:DatatypeProperty>

    <!-- http://schema.org/email -->

    <owl:DatatypeProperty rdf:about="http://schema.org/email">
      <rdfs:domain rdf:resource="http://schema.org/ContactPoint"/>
      <rdfs:range rdf:resource="http://www.w3.org/2001/XMLSchema#string"/>
      <rdfs:comment xml:lang="es">Correo electrónico de información.</rdfs:comment>
      <rdfs:comment xml:lang="en">E-mail from Contact Point</rdfs:comment>
      <rdfs:isDefinedBy rdf:resource="http://schema.org/"/>
      <rdfs:label xml:lang="es">Correo electrónico</rdfs:label>
      <rdfs:label xml:lang="en">E-mail</rdfs:label>
    </owl:DatatypeProperty>
    
    <!-- http://schema.org/endDate -->

    <owl:DatatypeProperty rdf:about="http://schema.org/endDate">
        <rdfs:domain rdf:resource="http://vocab.ciudadesabiertas.es/def/transporte/trafico#Incidencia"/>
        <rdfs:range rdf:resource="http://www.w3.org/2001/XMLSchema#dateTime"/>
        <rdfs:comment xml:lang="es">La fecha y hora de finalización de
	    una incidencia (en formato fecha ISO 8601)</rdfs:comment>
        <rdfs:comment xml:lang="en">The end date and time of an incidence (in ISO 8601 date format).</rdfs:comment>
        <rdfs:isDefinedBy rdf:resource="http://schema.org/"/>
        <rdfs:label xml:lang="en">end date</rdfs:label>
        <rdfs:label xml:lang="es">fecha de fin</rdfs:label>
    </owl:DatatypeProperty>

    <!-- http://schema.org/legalName -->

    <owl:DatatypeProperty rdf:about="http://schema.org/legalName">
      <rdfs:domain rdf:resource="http://schema.org/ContactPoint"/>
      <rdfs:range rdf:resource="http://www.w3.org/2001/XMLSchema#string"/>
      <rdfs:comment xml:lang="es">Nombre legal</rdfs:comment>
      <rdfs:comment xml:lang="en">Legal Name</rdfs:comment>
      <rdfs:isDefinedBy rdf:resource="http://schema.org/"/>
      <rdfs:label xml:lang="es">Legal Name</rdfs:label>
      <rdfs:label xml:lang="en">Nombre legal</rdfs:label>
    </owl:DatatypeProperty>

    <!-- http://schema.org/name -->

    <owl:DatatypeProperty rdf:about="http://schema.org/name">
      <rdfs:domain>
	<owl:Class>
	  <owl:unionOf rdf:parseType="Collection">
	    <rdf:Description rdf:about="http://w3id.org/transmodel/journeys#DayType"/>
	    <rdf:Description rdf:about="http://w3id.org/transmodel/journeys#LinkSequence"/>
	    <rdf:Description rdf:about="http://w3id.org/transmodel/journeys#Line"/>
	    <rdf:Description rdf:about="http://vocab.ciudadesabiertas.es/def/transporte/autobus#Parada"/>
	    <rdf:Description rdf:about="http://w3id.org/transmodel/journeys#ServiceCalendar"/>
	    <rdf:Description rdf:about="http://w3id.org/transmodel/journeys#StopArea"/>
	    <rdf:Description rdf:about="http://w3id.org/transmodel/commons#Zone"/>
	  </owl:unionOf>
	</owl:Class>
      </rdfs:domain>
      <rdfs:range rdf:resource="http://www.w3.org/2001/XMLSchema#string"/>
      <rdfs:comment xml:lang="es">Nombre</rdfs:comment>
      <rdfs:comment xml:lang="en">Name</rdfs:comment>
      <rdfs:isDefinedBy rdf:resource="http://schema.org/"/>
      <rdfs:label xml:lang="es">Name</rdfs:label>
      <rdfs:label xml:lang="en">Nombre</rdfs:label>
    </owl:DatatypeProperty>

    <!-- http://schema.org/startDate -->

    <owl:DatatypeProperty rdf:about="http://schema.org/startDate">
        <rdfs:domain rdf:resource="http://vocab.ciudadesabiertas.es/def/transporte/trafico#Incidencia"/>
        <rdfs:range rdf:resource="http://www.w3.org/2001/XMLSchema#dateTime"/>
        <rdfs:isDefinedBy rdf:resource="http://schema.org/"/>
        <rdfs:label xml:lang="en">(expected) start date</rdfs:label>
        <rdfs:comment xml:lang="es">La fecha y hora de inicio de una incidencia (en formato fecha ISO 8601).</rdfs:comment>
        <rdfs:comment xml:lang="en">The start date and time of an incidence (in ISO 8601 date format).</rdfs:comment>
        <rdfs:label xml:lang="es">fecha de inicio (prevista)</rdfs:label>
    </owl:DatatypeProperty>

    <!-- http://schema.org/telephone -->

    <owl:DatatypeProperty rdf:about="http://schema.org/telephone">
      <rdfs:domain rdf:resource="http://schema.org/ContactPoint"/>
      <rdfs:range rdf:resource="http://www.w3.org/2001/XMLSchema#string"/>
      <rdfs:comment xml:lang="es">Teléfono de información y contacto con la entidad</rdfs:comment>
      <rdfs:comment xml:lang="en">Telephone to contact and get some information from the entity </rdfs:comment>
      <rdfs:isDefinedBy rdf:resource="http://schema.org/"/>
      <rdfs:label xml:lang="es">Teléfono</rdfs:label>
      <rdfs:label xml:lang="en">Telephone</rdfs:label>
    </owl:DatatypeProperty>

    <!-- http://schema.org/url -->

    <owl:DatatypeProperty rdf:about="http://schema.org/url">
      <rdfs:domain>
	<owl:Class>
	  <owl:unionOf rdf:parseType="Collection">
	    <rdf:Description rdf:about="http://schema.org/ContactPoint"/>
	    <rdf:Description rdf:about="http://w3id.org/transmodel/journeys#Line"/>
	    <rdf:Description rdf:about="http://w3id.org/transmodel/journeys#Route"/>
	    <rdf:Description rdf:about="http://vocab.ciudadesabiertas.es/def/transporte/autobus#Parada"/>
	  </owl:unionOf>
	</owl:Class>
      </rdfs:domain>
      <rdfs:range rdf:resource="http://www.w3.org/2001/XMLSchema#anyURI"/>
      <rdfs:comment xml:lang="es">Public URL where you can get some information from the entity</rdfs:comment>
      <rdfs:comment xml:lang="en">Dirección URL pública donde puedes obtener información de la entidad</rdfs:comment>
      <rdfs:isDefinedBy rdf:resource="http://schema.org/"/>
      <rdfs:label xml:lang="es">URL</rdfs:label>
      <rdfs:label xml:lang="en">URL</rdfs:label>
    </owl:DatatypeProperty>

    <!-- http://www.w3.org/ns/sosa/resultTime -->

    <owl:DatatypeProperty rdf:about="http://www.w3.org/ns/sosa/resultTime">
        <rdfs:subPropertyOf rdf:resource="http://www.w3.org/2002/07/owl#topDataProperty"/>
        <rdfs:domain rdf:resource="http://vocab.ciudadesabiertas.es/def/transporte/autobus#RealTimePassingTime"/>
        <rdfs:range rdf:resource="http://www.w3.org/2001/XMLSchema#dateTime"/>
        <rdfs:comment xml:lang="es">Esta propiedad establece la fecha/hora de la observación.</rdfs:comment>
        <rdfs:comment xml:lang="en">This property sets the dateTime of the observation</rdfs:comment>
	
        <rdfs:label xml:lang="es">Hora Observación</rdfs:label>
        <rdfs:label xml:lang="en">Phenomenon Time</rdfs:label>
    </owl:DatatypeProperty>

    <!-- http://w3id.org/transmodel/commons#shortName -->

    <owl:DatatypeProperty rdf:about="http://w3id.org/transmodel/commons#shortName">
      <rdfs:subPropertyOf rdf:resource="http://www.w3.org/2002/07/owl#topDataProperty"/>
      <rdfs:domain>
	<owl:Class>
	  <owl:unionOf rdf:parseType="Collection">
	    <rdf:Description rdf:about="http://w3id.org/transmodel/journeys#Line"/>
	  </owl:unionOf>
	</owl:Class>
      </rdfs:domain>
        <rdfs:range rdf:resource="http://www.w3.org/2001/XMLSchema#string"/>
        <rdfs:comment xml:lang="en">Short name for an entity</rdfs:comment>
	<rdfs:comment xml:lang="es">Nombre corto para algo que lo necesite</rdfs:comment>
        <rdfs:label xml:lang="en">Short Name</rdfs:label>
	<rdfs:label xml:lang="es">Nombre corto</rdfs:label>
    </owl:DatatypeProperty>


    <!-- http://w3id.org/transmodel/journeys#date -->

    <owl:DatatypeProperty rdf:about="http://w3id.org/transmodel/journeys#date">
        <rdfs:subPropertyOf rdf:resource="http://www.w3.org/2002/07/owl#topDataProperty"/>
        <rdfs:domain rdf:resource="http://w3id.org/transmodel/journeys#DayTypeAssignment"/>
        <rdfs:range rdf:resource="http://www.w3.org/2001/XMLSchema#dateTime"/>
        <rdfs:comment xml:lang="en">Date of a Day Type Assignment.</rdfs:comment>
	<rdfs:comment xml:lang="es">Fecha de una Asignación de Día Tipo.</rdfs:comment>
        <rdfs:label xml:lang="en">Date</rdfs:label>
	<rdfs:label xml:lang="es">Fecha</rdfs:label>
    </owl:DatatypeProperty>
    

    <!-- http://w3id.org/transmodel/journeys#departureTime -->

    <owl:DatatypeProperty rdf:about="http://w3id.org/transmodel/journeys#departureTime">
        <rdfs:subPropertyOf rdf:resource="http://www.w3.org/2002/07/owl#topDataProperty"/>
        <rdfs:domain rdf:resource="http://w3id.org/transmodel/journeys#VehicleJourney"/>
        <rdfs:range rdf:resource="http://www.w3.org/2001/XMLSchema#dateTime"/>
        <rdfs:comment xml:lang="en">Departure time scheduled for a Vehicle Journey.</rdfs:comment>
	<rdfs:comment xml:lang="es">Hora de salida programada del viaje de un vehículo.</rdfs:comment>
        <rdfs:label xml:lang="en">Departure Time</rdfs:label>
	<rdfs:label xml:lang="es">Hora de salida</rdfs:label>
    </owl:DatatypeProperty>

    <!-- http://w3id.org/transmodel/journeys#earliestTime -->

    <owl:DatatypeProperty rdf:about="http://w3id.org/transmodel/journeys#earliestTime">
        <rdfs:subPropertyOf rdf:resource="http://www.w3.org/2002/07/owl#topDataProperty"/>
        <rdfs:domain rdf:resource="http://w3id.org/transmodel/journeys#DayType"/>
        <rdfs:range rdf:resource="http://www.w3.org/2001/XMLSchema#dateTime"/>
        <rdfs:comment xml:lang="en">Earliest time for the beginning of a service a certain Day Type.</rdfs:comment>
	<rdfs:comment xml:lang="es">Hora más temprana para el inicio de un servicio un cierto día tipo.</rdfs:comment>
        <rdfs:label xml:lang="en">Earliest Time</rdfs:label>
	<rdfs:label xml:lang="es">Hora más temprana</rdfs:label>
    </owl:DatatypeProperty>

    <!-- http://w3id.org/transmodel/journeys#distance -->

    <owl:DatatypeProperty rdf:about="http://w3id.org/transmodel/journeys#distance">
      <rdfs:subPropertyOf rdf:resource="http://www.w3.org/2002/07/owl#topDataProperty"/>
      <rdfs:domain rdf:resource="http://w3id.org/transmodel/journeys#LinkSequence"/>
      <rdfs:range rdf:resource="http://www.w3.org/2001/XMLSchema#double"/>
      <rdfs:comment xml:lang="en">Total distance for a Line or a Route like.</rdfs:comment>
      <rdfs:comment xml:lang="es">Distancia total para una Línea o una Ruta o similares.</rdfs:comment>
      <rdfs:label xml:lang="en">Distance</rdfs:label>
      <rdfs:label xml:lang="es">Distancia</rdfs:label>
    </owl:DatatypeProperty>

    <!-- http://w3id.org/transmodel/journeys#distanceFromStart -->

    <owl:DatatypeProperty rdf:about="http://w3id.org/transmodel/journeys#distanceFromStart">
      <rdfs:subPropertyOf rdf:resource="http://www.w3.org/2002/07/owl#topDataProperty"/>
      <rdfs:domain rdf:resource="http://w3id.org/transmodel/journeys#PointInLinkSequence"/>
      <rdfs:range rdf:resource="http://www.w3.org/2001/XMLSchema#double"/>
      <rdfs:comment xml:lang="en">For a Point in a Link Sequence (or alike), this property represents the distance from the start of the corresponding Journey Pattern or alike.</rdfs:comment>
      <rdfs:comment xml:lang="es">Para un Punto en una Secuencia de enlaces (o similares), esta propiedad representa la distancia desde el comienzo del correspondiente Patrón de Viaje o similares.</rdfs:comment>
      <rdfs:label xml:lang="en">Distance from start</rdfs:label>
      <rdfs:label xml:lang="es">Distancia desde el inicio</rdfs:label>
    </owl:DatatypeProperty>

    <!-- http://w3id.org/transmodel/journeys#firstDepartureTime -->

    <owl:DatatypeProperty rdf:about="http://w3id.org/transmodel/journeys#firstDepartureTime">
        <rdfs:subPropertyOf rdf:resource="http://www.w3.org/2002/07/owl#topDataProperty"/>
        <rdfs:domain rdf:resource="http://w3id.org/transmodel/journeys#HeadwayJourneyGroup"/>
        <rdfs:range rdf:resource="http://www.w3.org/2001/XMLSchema#dateTime"/>
        <rdfs:comment xml:lang="en">The time of beginning of a Vehicle Journey.</rdfs:comment>
	<rdfs:comment xml:lang="es">La hora de inicio de un Viaje de un Vehículo.</rdfs:comment>
        <rdfs:label xml:lang="en">First departure time</rdfs:label>
	<rdfs:label xml:lang="es">Primera hora de salida</rdfs:label>
    </owl:DatatypeProperty>

    <!-- http://w3id.org/transmodel/journeys#forAlighting -->

    <owl:DatatypeProperty rdf:about="http://w3id.org/transmodel/journeys#forAlighting">
        <rdfs:subPropertyOf rdf:resource="http://www.w3.org/2002/07/owl#topDataProperty"/>
        <rdfs:domain rdf:resource="http://w3id.org/transmodel/journeys#ScheduledStopPoint"/>
        <rdfs:range rdf:resource="http://www.w3.org/2001/XMLSchema#boolean"/>
        <rdfs:comment xml:lang="en">This property allows describing whether the stop may be used for alighting.</rdfs:comment>
	<rdfs:comment xml:lang="es">Esta propiedad indica si la parada se puede usar para bajarse o no.</rdfs:comment>
        <rdfs:label xml:lang="en">for Alighting</rdfs:label>
	<rdfs:label xml:lang="es">Para bajarse</rdfs:label>
    </owl:DatatypeProperty>
    
    <!-- http://w3id.org/transmodel/journeys#forBoarding -->

    <owl:DatatypeProperty rdf:about="http://w3id.org/transmodel/journeys#forBoarding">
        <rdfs:subPropertyOf rdf:resource="http://www.w3.org/2002/07/owl#topDataProperty"/>
        <rdfs:domain rdf:resource="http://w3id.org/transmodel/journeys#ScheduledStopPoint"/>
        <rdfs:range rdf:resource="http://www.w3.org/2001/XMLSchema#boolean"/>
        <rdfs:comment xml:lang="en">This property allows describing whether the stop may be used for boarding</rdfs:comment>
	<rdfs:comment xml:lang="es">Esta propiedad indica si se puede montar en la parada.</rdfs:comment>
        <rdfs:label xml:lang="en">for Boarding</rdfs:label>
	<rdfs:label xml:lang="es">para subirse</rdfs:label>
    </owl:DatatypeProperty>

    <!-- http://w3id.org/transmodel/journeys#from -->

    <owl:DatatypeProperty rdf:about="http://w3id.org/transmodel/journeys#from">
        <rdfs:subPropertyOf rdf:resource="http://www.w3.org/2002/07/owl#topDataProperty"/>
        <rdfs:domain rdf:resource="http://w3id.org/transmodel/journeys#ServiceCalendar"/>
        <rdfs:range rdf:resource="http://www.w3.org/2001/XMLSchema#date"/>
        <rdfs:comment xml:lang="en">This property allows describing the beginning of a Service Calendar</rdfs:comment>
	<rdfs:comment xml:lang="es">Esta propiedad permite describir el inicio de un calendario de servicio.</rdfs:comment>
        <rdfs:label xml:lang="en">from</rdfs:label>
	<rdfs:label xml:lang="es">desde</rdfs:label>
    </owl:DatatypeProperty>

    <!-- http://w3id.org/transmodel/journeys#frontText -->

    <owl:DatatypeProperty rdf:about="http://w3id.org/transmodel/journeys#frontText">
      <rdfs:domain rdf:resource="http://w3id.org/transmodel/journeys#DestinationDisplay"/>
      <rdfs:range rdf:resource="http://www.w3.org/2001/XMLSchema#string"/>
      <rdfs:comment xml:lang="en">Displayed Text usually in the front of a Vehicle of the Public Transport Service.</rdfs:comment>
      <rdfs:comment xml:lang="es">Texto que se muestra normalmente en la parte frontal de un vehículo del servicio público de transporte.</rdfs:comment>
      <rdfs:label xml:lang="en">Front Text</rdfs:label>
      <rdfs:label xml:lang="es">Letrero de Cabecera</rdfs:label>
    </owl:DatatypeProperty>

    <!-- http://w3id.org/transmodel/journeys#isAvailable -->

    <owl:DatatypeProperty rdf:about="http://w3id.org/transmodel/journeys#isAvailable">
        <rdfs:subPropertyOf rdf:resource="http://www.w3.org/2002/07/owl#topDataProperty"/>
        <rdfs:domain rdf:resource="http://w3id.org/transmodel/journeys#DayTypeAssignment"/>
        <rdfs:range rdf:resource="http://www.w3.org/2001/XMLSchema#boolean"/>
        <rdfs:comment xml:lang="en">Property to state whether the Day Type Assignment is available or not.</rdfs:comment>
	<rdfs:comment xml:lang="es">Propiedad que determina si una Asignación de Día Tipo está disponible o no..</rdfs:comment>
        <rdfs:label xml:lang="en">Is Available</rdfs:label>
	<rdfs:label xml:lang="es">Disponibilidad</rdfs:label>
    </owl:DatatypeProperty>

    <!-- http://w3id.org/transmodel/journeys#journeyDuration -->

    <owl:DatatypeProperty rdf:about="http://w3id.org/transmodel/journeys#journeyDuration">
        <rdfs:subPropertyOf rdf:resource="http://www.w3.org/2002/07/owl#topDataProperty"/>
        <rdfs:domain rdf:resource="http://w3id.org/transmodel/journeys#VehicleJourney"/>
        <rdfs:range rdf:resource="http://www.w3.org/2001/XMLSchema#dateTime"/>
        <rdfs:comment xml:lang="en">Journey duration scheduled for a Vehicle Journey.</rdfs:comment>
	<rdfs:comment xml:lang="es">Duración programada del viaje de un vehículo.</rdfs:comment>
        <rdfs:label xml:lang="en">Journey Duration</rdfs:label>
	<rdfs:label xml:lang="es">Duración del viaje</rdfs:label>
    </owl:DatatypeProperty>

    <!-- http://w3id.org/transmodel/journeys#lastDayOffset -->

    <owl:DatatypeProperty rdf:about="http://w3id.org/transmodel/journeys#lastDayOffset">
        <rdfs:subPropertyOf rdf:resource="http://www.w3.org/2002/07/owl#topDataProperty"/>
        <rdfs:domain rdf:resource="http://w3id.org/transmodel/journeys#HeadwayJourneyGroup"/>
        <rdfs:range rdf:resource="http://www.w3.org/2001/XMLSchema#dateTime"/>
        <rdfs:comment xml:lang="en">The offset time of ending of a Vehicle Journey.</rdfs:comment>
	<rdfs:comment xml:lang="es">La hora de ajuste del fin de un Viaje de un Vehículo.</rdfs:comment>
        <rdfs:label xml:lang="en">Last day offset</rdfs:label>
	<rdfs:label xml:lang="es">Ajuste de hora de la última salida</rdfs:label>
    </owl:DatatypeProperty>

    <!-- http://w3id.org/transmodel/journeys#lastDepartureTime -->

    <owl:DatatypeProperty rdf:about="http://w3id.org/transmodel/journeys#lastDepartureTime">
        <rdfs:subPropertyOf rdf:resource="http://www.w3.org/2002/07/owl#topDataProperty"/>
        <rdfs:domain rdf:resource="http://w3id.org/transmodel/journeys#HeadwayJourneyGroup"/>
        <rdfs:range rdf:resource="http://www.w3.org/2001/XMLSchema#dateTime"/>
        <rdfs:comment xml:lang="en">The time of ending of a Vehicle Journey.</rdfs:comment>
	<rdfs:comment xml:lang="es">La hora de fin de un Viaje de un Vehículo.</rdfs:comment>
        <rdfs:label xml:lang="en">last departure time</rdfs:label>
	<rdfs:label xml:lang="es">última hora de salida</rdfs:label>
    </owl:DatatypeProperty>

    
    <!-- http://w3id.org/transmodel/journeys#maximumHeadwayInterval -->

    <owl:DatatypeProperty rdf:about="http://w3id.org/transmodel/journeys#maximumHeadwayInterval">
        <rdfs:subPropertyOf rdf:resource="http://www.w3.org/2002/07/owl#topDataProperty"/>
        <rdfs:domain rdf:resource="http://w3id.org/transmodel/journeys#HeadwayInterval"/>
        <rdfs:range rdf:resource="http://www.w3.org/2001/XMLSchema#dateTime"/>
        <rdfs:comment xml:lang="en">The maximum interval from Headway.</rdfs:comment>
	<rdfs:comment xml:lang="es">Máximo intervalo/frecuencia fijada desde cabecera.</rdfs:comment>
        <rdfs:label xml:lang="en">Maximum Headway Interval</rdfs:label>
	<rdfs:label xml:lang="es">Frecuencia máxima</rdfs:label>
    </owl:DatatypeProperty>

    <!-- http://w3id.org/transmodel/journeys#minimumHeadwayInterval -->

    <owl:DatatypeProperty rdf:about="http://w3id.org/transmodel/journeys#minimumHeadwayInterval">
        <rdfs:subPropertyOf rdf:resource="http://www.w3.org/2002/07/owl#topDataProperty"/>
        <rdfs:domain rdf:resource="http://w3id.org/transmodel/journeys#HeadwayInterval"/>
        <rdfs:range rdf:resource="http://www.w3.org/2001/XMLSchema#dateTime"/>
        <rdfs:comment xml:lang="en">The minimum interval from Headway.</rdfs:comment>
	<rdfs:comment xml:lang="es">Mínimo intervalo/frecuencia fijada desde cabecera.</rdfs:comment>
        <rdfs:label xml:lang="en">Minimum Headway Interval</rdfs:label>
	<rdfs:label xml:lang="es">Frecuencia mínima</rdfs:label>
    </owl:DatatypeProperty>

    <!-- http://w3id.org/transmodel/journeys#minimumHeadwayInterval -->

    <owl:DatatypeProperty rdf:about="http://w3id.org/transmodel/journeys#scheduledHeadwayInterval">
        <rdfs:subPropertyOf rdf:resource="http://www.w3.org/2002/07/owl#topDataProperty"/>
        <rdfs:domain rdf:resource="http://w3id.org/transmodel/journeys#HeadwayInterval"/>
        <rdfs:range rdf:resource="http://www.w3.org/2001/XMLSchema#dateTime"/>
        <rdfs:comment xml:lang="en">The scheduled interval from Headway.</rdfs:comment>
	<rdfs:comment xml:lang="es">Intervalo/frecuencia programada desde cabecera.</rdfs:comment>
        <rdfs:label xml:lang="en">Scheduled Headway Interval</rdfs:label>
	<rdfs:label xml:lang="es">Frecuencia programada</rdfs:label>
    </owl:DatatypeProperty>

     <!-- http://w3id.org/transmodel/journeys#order -->

    <owl:DatatypeProperty rdf:about="http://w3id.org/transmodel/journeys#order">
      <rdfs:subPropertyOf rdf:resource="http://www.w3.org/2002/07/owl#topDataProperty"/>
      <rdfs:domain rdf:resource="http://w3id.org/transmodel/journeys#PointInLinkSequence"/>
        <rdfs:range rdf:resource="http://www.w3.org/2001/XMLSchema#nonNegativeInteger"/>
        <rdfs:comment xml:lang="en">Order of a Point in Link Sequence, or in a Point on Route within sequence, or in any other type of situation where the order or points are relevant</rdfs:comment>
	<rdfs:comment xml:lang="es">Orden de un Punto en una Secuencia de Enlaces (Link Sequence) y por tanto de un Punto en una Ruta o en cualquier otra estructura similar.</rdfs:comment>
        <rdfs:label xml:lang="en">Order</rdfs:label>
	<rdfs:label xml:lang="es">Orden</rdfs:label>
    </owl:DatatypeProperty>

    <!-- http://w3id.org/transmodel/journeys#to -->

    <owl:DatatypeProperty rdf:about="http://w3id.org/transmodel/journeys#to">
        <rdfs:subPropertyOf rdf:resource="http://www.w3.org/2002/07/owl#topDataProperty"/>
        <rdfs:domain rdf:resource="http://w3id.org/transmodel/journeys#ServiceCalendar"/>
        <rdfs:range rdf:resource="http://www.w3.org/2001/XMLSchema#date"/>
        <rdfs:comment xml:lang="en">This property allows describing the end of a Service Calendar</rdfs:comment>
	<rdfs:comment xml:lang="es">Esta propiedad permite describir el fin de un calendario de servicio.</rdfs:comment>
        <rdfs:label xml:lang="en">to</rdfs:label>
	<rdfs:label xml:lang="es">hasta</rdfs:label>
    </owl:DatatypeProperty>

    <!-- http://vocab.ciudadesabiertas.es/def/transporte/trafico#esRecurrente -->

    <owl:DatatypeProperty rdf:about="http://vocab.ciudadesabiertas.es/def/transporte/trafico#esRecurrente">
        <rdfs:subPropertyOf rdf:resource="http://www.w3.org/2002/07/owl#topDataProperty"/>
        <rdfs:domain rdf:resource="http://vocab.ciudadesabiertas.es/def/transporte/trafico#IncidenciaPlanificada"/>
        <rdfs:range rdf:resource="http://www.w3.org/2001/XMLSchema#boolean"/>
        <rdfs:comment xml:lang="es">Esta propiedad permite describir si la incidencia es recurrente o no.</rdfs:comment>
        <rdfs:comment xml:lang="en">This property allows describing whether there is a recurrence in the
	    incidence or not</rdfs:comment>
        <rdfs:label xml:lang="es">Incidencia recurrente</rdfs:label>
        <rdfs:label xml:lang="en">Recurrent incidence</rdfs:label>
    </owl:DatatypeProperty>

    <!-- http://vocab.ciudadesabiertas.es/def/transporte/trafico#fechaFinPrevista -->

    <owl:DatatypeProperty rdf:about="http://vocab.ciudadesabiertas.es/def/transporte/trafico#fechaFinPrevista">
        <rdfs:domain rdf:resource="http://vocab.ciudadesabiertas.es/def/transporte/trafico#IncidenciaPlanificada"/>
        <rdfs:range rdf:resource="http://www.w3.org/2001/XMLSchema#dateTime"/>
        <rdfs:comment xml:lang="es">La fecha y hora prevista de
	    finalización de una incidencia planificada (en formato fecha ISO 8601)</rdfs:comment>
        <rdfs:comment xml:lang="en">The end date and time of a planned
	    incidence (in ISO 8601 date format).</rdfs:comment>
        <rdfs:isDefinedBy rdf:resource="http://schema.org/"/>
        <rdfs:label xml:lang="en">(expected) end date</rdfs:label>
        <rdfs:label xml:lang="es">fecha de fin (prevista)</rdfs:label>
    </owl:DatatypeProperty>
    
    <!-- http://vocab.ciudadesabiertas.es/def/transporte/trafico#numCarriles -->

    <owl:DatatypeProperty rdf:about="http://vocab.ciudadesabiertas.es/def/transporte/trafico#numCarriles">
        <rdfs:domain rdf:resource="http://vocab.ciudadesabiertas.es/def/transporte/trafico#Incidencia"/>
        <rdfs:range rdf:resource="http://www.w3.org/2001/XMLSchema#integer"/>
        <rdfs:comment xml:lang="en">Number of lanes of traffic</rdfs:comment>
        <rdfs:comment xml:lang="es">Número de carriles de circulación</rdfs:comment>
        <rdfs:isDefinedBy rdf:resource="http://vocab.ciudadesabiertas.es/def/transporte/trafico"/>
        <rdfs:label xml:lang="es">Carriles de circulación</rdfs:label>
        <rdfs:label xml:lang="en">Traffic lanes</rdfs:label>
    </owl:DatatypeProperty>

    <!-- http://vocab.ciudadesabiertas.es/def/transporte/trafico#numSentidos -->

    <owl:DatatypeProperty rdf:about="http://vocab.ciudadesabiertas.es/def/transporte/trafico#numSentidos">
        <rdfs:domain rdf:resource="http://vocab.ciudadesabiertas.es/def/transporte/trafico#Incidencia"/>
        <rdfs:range rdf:resource="http://www.w3.org/2001/XMLSchema#integer"/>
        <rdfs:comment xml:lang="en">Number of directions of traffic</rdfs:comment>
        <rdfs:comment xml:lang="es">Número de sentidos de circulación</rdfs:comment>
        <rdfs:isDefinedBy rdf:resource="http://vocab.ciudadesabiertas.es/def/transporte/trafico"/>
        <rdfs:label xml:lang="es">Sentidos de circulación</rdfs:label>
        <rdfs:label xml:lang="en">Street directions</rdfs:label>
    </owl:DatatypeProperty>

    <!-- http://vocab.ciudadesabiertas.es/def/transporte/trafico#recurrencia -->

    <owl:DatatypeProperty rdf:about="http://vocab.ciudadesabiertas.es/def/transporte/trafico#recurrencia">
        <rdfs:subPropertyOf rdf:resource="http://www.w3.org/2002/07/owl#topDataProperty"/>
        <rdfs:domain rdf:resource="http://vocab.ciudadesabiertas.es/def/transporte/trafico#IncidenciaPlanificada"/>
        <rdfs:range rdf:resource="http://www.w3.org/2001/XMLSchema#string"/>
        <rdfs:comment xml:lang="es">Esta propiedad permite describir la recurrencia.</rdfs:comment>
        <rdfs:comment xml:lang="en">This property allows describing the recurrence</rdfs:comment>
        <rdfs:label xml:lang="en">Recurrence</rdfs:label>
        <rdfs:label xml:lang="es">Recurrencia</rdfs:label>
    </owl:DatatypeProperty>

    <!-- http://vocab.ciudadesabiertas.es/def/transporte/autobus#expectedArrivalTime -->
    <owl:DatatypeProperty rdf:about="http://vocab.ciudadesabiertas.es/def/transporte/autobus#expectedArrivalTime">
        <rdfs:subPropertyOf rdf:resource="http://www.w3.org/2002/07/owl#topDataProperty"/>
        <rdfs:domain rdf:resource="http://vocab.ciudadesabiertas.es/def/transporte/autobus#RealTimePassingTime"/>
        <rdfs:range rdf:resource="http://www.w3.org/2001/XMLSchema#duration"/>
        <rdfs:comment xml:lang="en">Expecected arrival time of a Bus at a Stop Place, esautob:RealTimePassingTime.</rdfs:comment>
	<rdfs:comment xml:lang="es">Tiempo de llegada prevista para un autobús en una parada, duración de esautob:RealTimePassingTime</rdfs:comment>
        <rdfs:label xml:lang="en">Expected Arrival Time</rdfs:label>
	<rdfs:label xml:lang="es">Tiempo de llegada previsto</rdfs:label>
    </owl:DatatypeProperty>


    <!-- http://vocab.ciudadesabiertas.es/def/transporte/autobus#panelElectronico -->

    <owl:DatatypeProperty rdf:about="http://vocab.ciudadesabiertas.es/def/transporte/autobus#panelElectronico">
        <rdfs:subPropertyOf rdf:resource="http://www.w3.org/2002/07/owl#topDataProperty"/>
        <rdfs:domain rdf:resource="http://vocab.ciudadesabiertas.es/def/transporte/autobus#Parada"/>
        <rdfs:range rdf:resource="http://www.w3.org/2001/XMLSchema#boolean"/>
        <rdfs:comment xml:lang="es">La Parada dispone de un Panel Electrónico Informativo que permite dar información actualizada de tiempos de llegada y otros.</rdfs:comment>
        <rdfs:comment xml:lang="en">The Stop Place has an Electronic Information Panel to display information up to date of the waiting time and othe kind of information if necessary.</rdfs:comment>
        <rdfs:label xml:lang="en">Electronic Information Panel</rdfs:label>
        <rdfs:label xml:lang="es">Panel Electrónico Informativo</rdfs:label>
    </owl:DatatypeProperty>

    <!-- http://vocab.ciudadesabiertas.es/def/transporte/autobus#wifi -->

    <owl:DatatypeProperty rdf:about="http://vocab.ciudadesabiertas.es/def/transporte/autobus#wifi">
        <rdfs:subPropertyOf rdf:resource="http://www.w3.org/2002/07/owl#topDataProperty"/>
        <rdfs:domain rdf:resource="http://vocab.ciudadesabiertas.es/def/transporte/autobus#Parada"/>
        <rdfs:range rdf:resource="http://www.w3.org/2001/XMLSchema#boolean"/>
        <rdfs:comment xml:lang="es">La parada dispone de conexión Wifi pública.</rdfs:comment>
        <rdfs:comment xml:lang="en">The Stop Place has a public WiFi network.</rdfs:comment>
        <rdfs:label xml:lang="en">WiFi</rdfs:label>
        <rdfs:label xml:lang="es">Wifi</rdfs:label>
    </owl:DatatypeProperty>

    <!-- http://vocab.ciudadesabiertas.es/def/transporte/autobus#zona -->

    <owl:DatatypeProperty rdf:about="http://vocab.ciudadesabiertas.es/def/transporte/autobus#zona">
        <rdfs:subPropertyOf rdf:resource="http://www.w3.org/2002/07/owl#topDataProperty"/>
        <rdfs:domain rdfs:resource="http://vocab.ciudadesabiertas.es/def/transporte/autobus#Parada"/>
        <rdfs:range rdf:resource="http://www.w3.org/2001/XMLSchema#string"/>
        <rdfs:comment xml:lang="es">Zona a la que pertenece la Parada.</rdfs:comment>
        <rdfs:comment xml:lang="en">The Stop Place is part of a Zone.</rdfs:comment>
        <rdfs:label xml:lang="en">Zone</rdfs:label>
        <rdfs:label xml:lang="es">Zona</rdfs:label>
    </owl:DatatypeProperty>

    <!-- http://w3id.org/transmodel/commons#colour -->

    <owl:DatatypeProperty rdf:about="http://w3id.org/transmodel/commons#colour">
      <rdfs:domain rdf:resource="http://w3id.org/transmodel/commons#Presentation"/>
      <rdfs:range rdf:resource="http://www.w3.org/2001/XMLSchema#string"/>
      <rdfs:comment xml:lang="en">The colour used to represent something with a Presentation (e.g., a Line)</rdfs:comment>
      <rdfs:comment xml:lang="es">Esta propiedad permite describir el color de algo que va en Presentación de información, como por ejemplo el color identificativo de una lína.</rdfs:comment>
      <rdfs:label xml:lang="en">colour</rdfs:label>
      <rdfs:label xml:lang="es">color</rdfs:label>
    </owl:DatatypeProperty>
    
    <!-- http://w3id.org/transmodel/commons#textColour -->

    <owl:DatatypeProperty rdf:about="http://w3id.org/transmodel/commons#textColour">
      <rdfs:domain rdf:resource="http://w3id.org/transmodel/commons#Presentation"/>
      <rdfs:range rdf:resource="http://www.w3.org/2001/XMLSchema#string"/>
      <rdfs:comment xml:lang="en">The colour used to represent the text associated to something with a Presentation (e.g., a Line)</rdfs:comment>
      <rdfs:comment xml:lang="es">El color que se usa para representar el texto asociado con una Presentación, por ejemplo de una línea.</rdfs:comment>
      <rdfs:label xml:lang="en">text colour</rdfs:label>
      <rdfs:label xml:lang="es">color de texto</rdfs:label>
    </owl:DatatypeProperty>

    
    <!-- 
	 ///////////////////////////////////////////////////////////////////////////////////////
	 // // Classes  //
	 ///////////////////////////////////////////////////////////////////////////////////////
    -->


    <!-- http://www.w3.org/ns/org#Organization -->

    <owl:Class rdf:about="http://www.w3.org/ns/org#Organization">
      <rdfs:comment xml:lang="en">Represents a collection of people organized together into a community or other social, commercial or political structure. The group has some common purpose or reason for existence which goes beyond the set of people belonging to it and can act as an Agent. Organizations are often decomposable into hierarchical structures.  It is recommended that SKOS lexical labels should be used to label the Organization. In particular `skos:prefLabel` for the primary (possibly legally recognized name), `skos:altLabel` for alternative names (trading names, colloquial names) and `skos:notation` to denote a code from a code list. Alternative names: _Collective_ _Body_ _Org_ _Group_</rdfs:comment>
      <rdfs:comment xml:lang="es">Grupo de personas que se organiza en una comunidad u otro tipo de estructura social, comercial o política. Dicho grupo tiene un objetivo o motivo común para su existencia que va más allá del conjunto de personas que lo forman y que puede actuar como “agente”. A menudo las organizaciones se pueden agrupar en estructuras jerárquicas. Se recomienda el uso de etiquetas de SKOS para denominar a cada “organización”. En concreto, `skos:prefLabel` para la denominación principal o recomendada (aquella reconocida legalmente, siempre que sea posible), `skos:altLabel` para denominaciones alternativas (nombre comercial, sigla, denominación por la que se conoce a la organización coloquialmente) y `skos:notation` para referirse al código que identifique a la organización en una lista de códigos. Denominaciones alternativas: _colectivo_ _corporación_ _grupo_.</rdfs:comment>
      <rdfs:label xml:lang="en">Organization</rdfs:label>
      <rdfs:label xml:lang="es">Organización</rdfs:label>
    </owl:Class>

    <!-- http://vocab.ciudadesabiertas.es/def/transporte/autobus#Linea -->

    <owl:Class rdf:about="http://vocab.ciudadesabiertas.es/def/transporte/autobus#Linea">
      <rdfs:subClassOf rdf:resource="http://w3id.org/transmodel/journeys#Line"/>
      <owl:disjointWith rdf:resource="http://w3id.org/transmodel/journeys#JourneyPattern"/>
        <rdfs:comment xml:lang="es">Línea del servicio público de transporte de autobuses urbanos</rdfs:comment>
        <rdfs:comment xml:lang="en">Line of the public transport service of urban buses</rdfs:comment>
        <rdfs:isDefinedBy rdf:resource="http://vocab.ciudadesabiertas.es/def/transporte/autobus"/>
        <rdfs:label xml:lang="es">Línea de autobús</rdfs:label>
        <rdfs:label xml:lang="en">Bus Line</rdfs:label>
    </owl:Class>

    <!-- http://vocab.ciudadesabiertas.es/def/transporte/autobus#Parada -->

    <owl:Class rdf:about="http://vocab.ciudadesabiertas.es/def/transporte/autobus#Parada">
      <rdfs:subClassOf rdf:resource="http://w3id.org/transmodel/commons#Place"/>
      <rdfs:subClassOf rdf:resource="http://www.opengis.net/ont/geosparql#Feature"/>
      <owl:disjointWith rdf:resource="http://vocab.ciudadesabiertas.es/def/transporte/trafico#Incidencia"/>
      <rdfs:comment xml:lang="en">A Stop of the public transport service of urban buses</rdfs:comment>
      <rdfs:comment xml:lang="es">Una parada del servicio público de transporte de autobuses urbanos.</rdfs:comment>
      <rdfs:isDefinedBy rdf:resource="http://vocab.ciudadesabiertas.es/def/transporte/trafico"/>
      <rdfs:label xml:lang="es">Parada</rdfs:label>
      <rdfs:label xml:lang="en">Stop Place</rdfs:label>
    </owl:Class>

    <!-- http://vocab.ciudadesabiertas.es/def/transporte/autobus#RealTimePassingTime -->

    <owl:Class rdf:about="http://vocab.ciudadesabiertas.es/def/transporte/autobus#RealTimePassingTime">
      <rdfs:subClassOf rdf:resource="http://www.w3.org/ns/sosa/Observation"/>
      <rdfs:comment xml:lang="en">Waiting time up to date</rdfs:comment>
	<rdfs:comment xml:lang="es">Tiempo de espera actualizado</rdfs:comment>
	<rdfs:isDefinedBy rdf:resource="http://vocab.ciudadesabiertas.es/def/transporte/trafico"/>
	<rdfs:label xml:lang="en">Waiting Time</rdfs:label>
	<rdfs:label xml:lang="es">Tiempo de Espera</rdfs:label>
    </owl:Class>

    <!-- Transmodel -->

    <!-- http://w3id.org/transmodel/journeys#DayType -->

    <owl:Class rdf:about="http://w3id.org/transmodel/journeys#DayType">
      <rdfs:comment xml:lang="en">A DayType is a type of day characterised by one or more properties which affect public transport operation</rdfs:comment>
      <rdfs:comment xml:lang="es">Un día tipo es un tipo de día caracterizado por una o más propiedades que afectan al transporte público</rdfs:comment>
      <rdfs:label xml:lang="en">DayType</rdfs:label>
      <rdfs:label xml:lang="es">Día Tipo</rdfs:label> 
    </owl:Class>

    <!-- http://w3id.org/transmodel/journeys#DayTypeAssignment -->

    <owl:Class rdf:about="http://w3id.org/transmodel/journeys#DayTypeAssignment">
      <rdfs:comment xml:lang="en">The assignment of operational characteristics, expressed by DAY TYPEs, to particular OPERATING DAYs within a SERVICE CALENDAR.</rdfs:comment>
      <rdfs:comment xml:lang="es">La asignación de características operativas, expresadas por Día Tipo, a un Día Operativo de un Calendario de Servicio.</rdfs:comment>
      <rdfs:label xml:lang="en">DayTypeAssignment</rdfs:label>
      <rdfs:label xml:lang="es">Asignación de Día Tipo</rdfs:label>
    </owl:Class>

    <!-- http://w3id.org/transmodel/journeys#DestinationDisplay -->

    <owl:Class rdf:about="http://w3id.org/transmodel/journeys#DestinationDisplay">
      <rdfs:comment xml:lang="en">An advertised destination of a specific Journey Pattern usually displayed on a headsign or other on-board locations</rdfs:comment>
      <rdfs:comment xml:lang="es">Un destino anunciado como un Patrón de Viaje específico normalmente mostrado en el frente del vehículo o en otros emplazamientos.</rdfs:comment>
      <rdfs:label xml:lang="en">Destination Display</rdfs:label>
      <rdfs:label xml:lang="es">Anuncio del Destino</rdfs:label>
    </owl:Class>

    <!-- http://w3id.org/transmodel/journeys#HeadwayInterval -->

    <owl:Class rdf:about="http://w3id.org/transmodel/journeys#HeadwayInterval">
        <rdfs:comment xml:lang="en">A time interval or a duration defining a headway period and characterizing HeadwayJourneyGroup</rdfs:comment>
	<rdfs:comment xml:lang="es">Un intervalo o duración determinada para una cabecera de línea que caracteriza el grupo de viajes desde cabecera de línea</rdfs:comment>
        <rdfs:label xml:lang="en">Headway Interval</rdfs:label>
	<rdfs:label xml:lang="es">Intervalo o frecuencia</rdfs:label>
    </owl:Class> 

    <!-- http://w3id.org/transmodel/journeys#HeadwayJourneyGroup -->

    <owl:Class rdf:about="http://w3id.org/transmodel/journeys#HeadwayJourneyGroup">
	<rdfs:comment xml:lang="en">A group of VEHICLE JOURNEYs following the same JOURNEY PATTERN having the same HEADWAY INTERVAL between a specified start and end time (for example, every 10 min). This is especially useful for passenger information.</rdfs:comment>
	<rdfs:comment xml:lang="es">Un grupo de viajes de vehículos que siguen el mismo intervalo fijado en cabecera entre el principio y el final (por ejemplo, cada 10 minutos). Esto es muy útil para los pasajeros.</rdfs:comment>
        <rdfs:label xml:lang="en">Headway Journey Group</rdfs:label>
	<rdfs:label xml:lang="es">Grupo de viajes con un horario</rdfs:label>
    </owl:Class>
    
    <!-- http://w3id.org/transmodel/journeys#JourneyPattern -->

    <owl:Class rdf:about="http://w3id.org/transmodel/journeys#JourneyPattern">
      <rdfs:subClassOf rdf:resource="http://w3id.org/transmodel/journeys#LinkSequence"/>
      <owl:disjointWith rdf:resource="http://vocab.ciudadesabiertas.es/def/transporte/autobus#Linea"/>
      <rdfs:comment xml:lang="en">An ordered list of Scheduled Stop Points and Timing Point on a single Route, describing the pattern of working for public transport vehicles. A Journey Pattern may pass through the same Point more than once. The first point of a JourneyPattern is the origin. The last point is the destination.</rdfs:comment>
      <rdfs:comment xml:lang="en">Una lista ordenada de paradas planificadas y puntos de control en una ruta que describe el patrón de funcionamiento de los vehículos de transporte públicos. Un patrón de viaje puede pasar por el mismo punto más de una vez. El primer punto del patrón es el origen y el último punto el destino.</rdfs:comment>
      <rdfs:label xml:lang="en">JourneyPattern</rdfs:label>
      <rdfs:label xml:lang="es">Patrón de viaje</rdfs:label>
    </owl:Class>

    <!-- http://w3id.org/transmodel/journeys#Line -->

    <owl:Class rdf:about="http://w3id.org/transmodel/journeys#Line">
        <rdfs:subClassOf>
            <owl:Restriction>
                <owl:onProperty rdf:resource="http://w3id.org/transmodel/journeys#presentedBy"/>
                <owl:allValuesFrom rdf:resource="http://w3id.org/transmodel/commons#Presentation"/>
            </owl:Restriction>
        </rdfs:subClassOf>
        <rdfs:comment xml:lang="en">A Line is a group of Routes which is generally known to the public by a similar name or number.</rdfs:comment>
	<rdfs:comment xml:lang="es">Una Línea es un grupo de Rutas que normalente se conocen por un nombre o número.</rdfs:comment>
        <rdfs:label xml:lang="en">Line</rdfs:label>
	<rdfs:label xml:lang="es">Línea</rdfs:label>
    </owl:Class>

    <!-- http://w3id.org/transmodel/journeys#LinkSequence -->

    <owl:Class rdf:about="http://w3id.org/transmodel/journeys#LinkSequence">
        <rdfs:subClassOf>
            <owl:Restriction>
                <owl:onProperty rdf:resource="http://w3id.org/transmodel/journeys#madeUpOf"/>
                <owl:allValuesFrom rdf:resource="http://w3id.org/transmodel/journeys#PointInLinkSequence"/>
            </owl:Restriction>
        </rdfs:subClassOf>
        <rdfs:comment xml:lang="en">An ordered sequence either of POINTs or of LINKs, defining a path through the network</rdfs:comment>
	<rdfs:comment xml:lang="es">Una secuencia ordenada de puntos o enlaces que definen una ruta a través de la red.</rdfs:comment>
	<rdfs:label xml:lang="es">Secuencia de enlaces</rdfs:label>
        <rdfs:label xml:lang="en">Link Sequence</rdfs:label>
    </owl:Class>


    <!-- http://w3id.org/transmodel/journeys#Point -->

    <owl:Class rdf:about="http://w3id.org/transmodel/journeys#Point">
      <rdfs:comment xml:lang="en">A Point is a 0-dimensional Node of the Network used for the spatial description of the network. Point may be located by a Location</rdfs:comment>
      <rdfs:comment xml:lang="es">Un punto topológico tiene dimensión 0, es un nodo de la red de transporte usado para la descripción espacial de la red. Puede ser localizado por una Ubicación.</rdfs:comment>
      <rdfs:label xml:lang="en">Point</rdfs:label>
      <rdfs:label xml:lang="es">Punto</rdfs:label>
    </owl:Class>

    <!-- http://w3id.org/transmodel/journeys#PointInJourneyPattern -->

    <owl:Class rdf:about="http://w3id.org/transmodel/journeys#PointInJourneyPattern">
        <rdfs:subClassOf rdf:resource="http://w3id.org/transmodel/journeys#PointInLinkSequence"/>
        <rdfs:subClassOf>
            <owl:Restriction>
                <owl:onProperty rdf:resource="http://w3id.org/transmodel/journeys#prescribing"/>
                <owl:allValuesFrom rdf:resource="http://w3id.org/transmodel/journeys#DestinationDisplay"/>
            </owl:Restriction>
        </rdfs:subClassOf>
        <rdfs:comment xml:lang="en">A Scheduled Stop Point OR Timing Point in a Journey Pattern with its order in that Journey Pattern</rdfs:comment>
	<rdfs:comment xml:lang="es">Una Parada Programada o un Punto de Control en un patrón de viaje con su orden en ese patrón.</rdfs:comment>
        <rdfs:label xml:lang="en">Point In Journey Pattern</rdfs:label>
	<rdfs:label xml:lang="es">Punto en un Patrón de Viaje</rdfs:label>
    </owl:Class>
    
    <!-- http://w3id.org/transmodel/journeys#PointInLinkSequence -->

    <owl:Class rdf:about="http://w3id.org/transmodel/journeys#PointInLinkSequence">
        <rdfs:subClassOf>
            <owl:Restriction>
                <owl:onProperty rdf:resource="http://w3id.org/transmodel/journeys#distanceFromStart"/>
                <owl:qualifiedCardinality rdf:datatype="http://www.w3.org/2001/XMLSchema#nonNegativeInteger">1</owl:qualifiedCardinality>
                <owl:onDataRange rdf:resource="http://www.w3.org/2001/XMLSchema#float"/>
            </owl:Restriction>
        </rdfs:subClassOf>
	<rdfs:subClassOf>
            <owl:Restriction>
                <owl:onProperty rdf:resource="http://w3id.org/transmodel/journeys#viewedAs"/>
                <owl:qualifiedCardinality rdf:datatype="http://www.w3.org/2001/XMLSchema#nonNegativeInteger">1</owl:qualifiedCardinality>
                <owl:onClass rdf:resource="http://w3id.org/transmodel/journeys#Point"/>
            </owl:Restriction>
        </rdfs:subClassOf>
	<rdfs:subClassOf>
            <owl:Restriction>
                <owl:onProperty rdf:resource="http://w3id.org/transmodel/journeys#order"/>
                <owl:qualifiedCardinality rdf:datatype="http://www.w3.org/2001/XMLSchema#nonNegativeInteger">1</owl:qualifiedCardinality>
                <owl:onDataRange rdf:resource="http://www.w3.org/2001/XMLSchema#nonNegativeInteger"/>
            </owl:Restriction>
        </rdfs:subClassOf>
        <rdfs:comment xml:lang="en">A POINT in a LINK SEQUENCE indicating its order in that particular LINK SEQUENCE.</rdfs:comment>
	<rdfs:comment xml:lang="es">Un punto en una secuencia indica su orden en esa secuencia de enlaces</rdfs:comment>
	<rdfs:label xml:lang="en">Point in Link Sequence</rdfs:label>
	<rdfs:label xml:lang="es">Punto en secuencia de enlaces</rdfs:label>
    </owl:Class>

        <!-- http://w3id.org/transmodel/journeys#PointOnRoute -->

    <owl:Class rdf:about="http://w3id.org/transmodel/journeys#PointOnRoute">
        <rdfs:subClassOf rdf:resource="http://w3id.org/transmodel/journeys#PointInLinkSequence"/>
        <rdfs:comment xml:lang="en">A Route Point used to define a Route with its order on that Route.</rdfs:comment>
	<rdfs:comment xml:lang="es">Un Punto de Ruta se usa para definir una Ruta con su orden en esa Ruta.</rdfs:comment>
        <rdfs:label xml:lang="en">Point on Route</rdfs:label>
	<rdfs:label xml:lang="es">Punto en la ruta</rdfs:label> 
    </owl:Class>


    <!-- http://w3id.org/transmodel/journeys#Route -->

    <owl:Class rdf:about="http://w3id.org/transmodel/journeys#Route">
      <rdfs:subClassOf rdf:resource="http://w3id.org/transmodel/journeys#LinkSequence"/>
      <rdfs:subClassOf>
        <owl:Restriction>
          <owl:onProperty rdf:resource="http://w3id.org/transmodel/journeys#directionType"/>
                <owl:allValuesFrom>
                    <owl:Class>
                        <owl:intersectionOf rdf:parseType="Collection">
                            <rdf:Description rdf:about="http://www.w3.org/2004/02/skos/core#Concept"/>
                            <owl:Restriction>
                                <owl:onProperty rdf:resource="http://www.w3.org/2004/02/skos/core#inScheme"/>
                                <owl:hasValue rdf:resource="http://w3id.org/transmodel/kos/journeys/direction-type"/>
                            </owl:Restriction>
                        </owl:intersectionOf>
                    </owl:Class>
                </owl:allValuesFrom>
            </owl:Restriction>
        </rdfs:subClassOf>
        <rdfs:comment xml:lang="en">A Route is and ordered list of located Points defining one single path through the road (or rail) network.</rdfs:comment>
	<rdfs:comment xml:lang="es">Una ruta es una lista ordenada de Puntos que definen una sola ruta a través de una red de calles</rdfs:comment>
        <rdfs:label xml:lang="en">Route</rdfs:label>
	<rdfs:label xml:lang="es">Ruta</rdfs:label>
    </owl:Class>
    
 <!-- http://w3id.org/transmodel/journeys#RoutePoint -->

    <owl:Class rdf:about="http://w3id.org/transmodel/journeys#RoutePoint">
        <rdfs:subClassOf rdf:resource="http://w3id.org/transmodel/journeys#Point"/>
        <rdfs:comment xml:lang="en">A Point used to define the shape of a Route through the network.</rdfs:comment>
	<rdfs:comment xml:lang="es">Un punto que se usa para definir la forma de una ruta por la red de transporte.</rdfs:comment>
        <rdfs:label xml:lang="en">Route Point</rdfs:label>
	<rdfs:label xml:lang="es">Punto de Ruta</rdfs:label>
    </owl:Class>
    <!-- http://w3id.org/transmodel/journeys#ScheduledStopPoint -->

    <owl:Class rdf:about="http://w3id.org/transmodel/journeys#ScheduledStopPoint">
      <rdfs:subClassOf rdf:resource="http://w3id.org/transmodel/journeys#Point"/>
      <rdfs:comment xml:lang="en">A Scheduled Stop Point is a Point where a Passenger can board or alight from a Vehicle.</rdfs:comment>
      <rdfs:comment xml:lang="es">Una Parada Planificada es un Punto donde se puede tomar o dejar un vehículo.</rdfs:comment>
      <rdfs:label xml:lang="en">Scheduled Stop Point</rdfs:label>
      <rdfs:label xml:lang="es">Parada Planificada</rdfs:label>
    </owl:Class>

    <!--  http://w3id.org/transmodel/journeys#ServiceCalendar -->

    <owl:Class rdf:about="http://w3id.org/transmodel/journeys#ServiceCalendar">
      <rdfs:label xml:lang="en">ServiceCalendar</rdfs:label>
      <rdfs:label xml:lang="es">Calendario de servicio</rdfs:label>
      <rdfs:comment xml:lang="en">A collection of DAY TYPE ASSIGNMENTs.</rdfs:comment>
      <rdfs:comment xml:lang="es">Un conjunto de tareas de un día tipo.</rdfs:comment>
    </owl:Class>

    <!-- http://w3id.org/transmodel/journeys#StopArea -->

    <owl:Class rdf:about="http://w3id.org/transmodel/journeys#StopArea">
        <rdfs:subClassOf rdf:resource="http://w3id.org/transmodel/commons#Place"/>
        <rdfs:comment xml:lang="en">A group of Scheduled Stop Points close to each other</rdfs:comment>
	<rdfs:comment xml:lang="es">Un grupo de Paradas que están próximas entre sí.</rdfs:comment>
        <rdfs:label xml:lang="en">Stop Area</rdfs:label>
	<rdfs:label xml:lang="es">Paradas</rdfs:label>
    </owl:Class>

    <!-- http://w3id.org/transmodel/journeys#StopPointInJourneyPattern -->

    <owl:Class rdf:about="http://w3id.org/transmodel/journeys#StopPointInJourneyPattern">
        <rdfs:subClassOf rdf:resource="http://w3id.org/transmodel/journeys#PointInJourneyPattern"/>
        <rdfs:comment xml:lang="en">A Point in Journey Pattern that is a Scheduled Stop Point</rdfs:comment>
	<rdfs:comment xml:lang="es">Un Punto en el Patrón de Viaje que se ve como una Parada Planificada</rdfs:comment>
        <rdfs:label xml:lang="en">Stop Point In Journey Pattern</rdfs:label>
	<rdfs:label xml:lang="es">Parada en Patrón de Viaje</rdfs:label>
    </owl:Class>


    <!-- http://w3id.org/transmodel/journeys#TimingPointInJourneyPattern -->

    <owl:Class rdf:about="http://w3id.org/transmodel/journeys#TimingPointInJourneyPattern">
        <rdfs:subClassOf rdf:resource="http://w3id.org/transmodel/journeys#Point"/>
	<rdfs:subClassOf rdf:resource="http://w3id.org/transmodel/journeys#PointInLinkSequence"/> <!-- check -->
        <rdfs:comment xml:lang="en">A Point in a JourneyPattern which is a TimingPoint</rdfs:comment>
	<rdfs:comment xml:lang="es">Un punto en un patrón de viaje que es un punto de control</rdfs:comment>
        <rdfs:label xml:lang="en">Timing Point In Journey Pattern</rdfs:label>
	<rdfs:label xml:lang="es">Punto de control en el patrón de viaje</rdfs:label>
    </owl:Class>

    <!-- http://w3id.org/transmodel/journeys#VehicleJourney -->

    <owl:Class rdf:about="http://w3id.org/transmodel/journeys#VehicleJourney">
	<rdfs:comment xml:lang="en">The planned movement of a Public Transport Vehicle on a DayType from the start point to the end point of a JourneyPattern on a specified Route.</rdfs:comment>
	<rdfs:comment xml:lang="es">El movimiento planificado de un vehículo de transporte público en un día tipo DayType desde un punto inicial al punto final de un patrón de viaje JourneyPattern en una ruta especificada.</rdfs:comment>
	<rdfs:label xml:lang="en">VehicleJourney</rdfs:label>
	<rdfs:label xml:lang="es">Viaje de un vehículo</rdfs:label>
    </owl:Class>

        <!-- http://w3id.org/transmodel/commons#Place -->

	<owl:Class rdf:about="http://w3id.org/transmodel/commons#Place">
	  <rdfs:subClassOf rdf:resource="http://w3id.org/transmodel/commons#Zone"/>
	  <rdfs:comment xml:lang="en">A geographic Place of any type which may be specified as the origin or destination of a Trip. A Place may be represented as a Point (dimension 0), a Road section (dimension 1) or a Zone (dimension 2)</rdfs:comment>
	  <rdfs:comment xml:lang="es">Un lugar geográfico de cualquier tipo que puede usarse como el origen o el destino de un Viaje. Debe representarse por un Punto (dimensión 0 en topología), una ruta (una dimensión en topología) o una zona (dos dimensiones en topología).</rdfs:comment>
	  <rdfs:label xml:lang="en">Place</rdfs:label>
	  <rdfs:label xml:lang="es">Lugar</rdfs:label>
	</owl:Class>
    
        <!-- http://w3id.org/transmodel/commons#Presentation -->

    <owl:Class rdf:about="http://w3id.org/transmodel/commons#Presentation">
        <rdfs:subClassOf>
            <owl:Restriction>
                <owl:onProperty rdf:resource="http://w3id.org/transmodel/commons#colour"/>
                <owl:allValuesFrom rdf:resource="http://www.w3.org/2001/XMLSchema#string"/>
            </owl:Restriction>
        </rdfs:subClassOf>
        <rdfs:subClassOf>
            <owl:Restriction>
                <owl:onProperty rdf:resource="http://w3id.org/transmodel/commons#textColour"/>
                <owl:allValuesFrom rdf:resource="http://www.w3.org/2001/XMLSchema#string"/>
            </owl:Restriction>
        </rdfs:subClassOf>
        <rdfs:comment xml:lang="en">This class is used to represent a Line, or any other object, in a map</rdfs:comment>
	<rdfs:comment xml:lang="es">Se utiliza para representar una Línea o cualquier otro objeto en un mapa.</rdfs:comment>
        <rdfs:label xml:lang="en">Presentation</rdfs:label>
	<rdfs:label xml:lang="es">Presentación</rdfs:label>
    </owl:Class>

        <!-- http://w3id.org/transmodel/commons#Zone -->

    <owl:Class rdf:about="http://w3id.org/transmodel/commons#Zone">
        <rdfs:comment xml:lang="en">A two-dimensional PLACE within the service area of a public transport operator (administrative zone, TARIFF ZONE, ACCESS ZONE, etc.).</rdfs:comment>
	<rdfs:comment xml:lang="es">La Zona es un Lugar (Place) de dos dimensiones que ese encuentra en el área que sirve un operador de transporte público. Puede ser una zona administrativa, una zona tarifaria, una zona de acceso o algo más concreto.</rdfs:comment>
        <rdfs:label xml:lang="en">Zone</rdfs:label>
	<rdfs:label xml:lang="es">Zona</rdfs:label>
    </owl:Class>

    <!-- http://w3id.org/transmodel/organisations#Authority -->

    <owl:Class rdf:about="http://w3id.org/transmodel/organisations#Authority">
        <rdfs:subClassOf rdf:resource="http://w3id.org/transmodel/organisations#Organisation"/>
        <owl:disjointWith rdf:resource="http://w3id.org/transmodel/organisations#Organisation"/>
        <rdfs:comment xml:lang="en">Public Transport Authority, the organization under which the responsability of organising the TransportService in a certain area (AdministrativeZone) is placed</rdfs:comment>
	<rdfs:comment xml:lang="es">Autoridad del Transporte Público, organización bajo la cual está la responsabilidad de organizar el servicio de transporte de una cierta área (por ejemplo, zona administrativa).</rdfs:comment>
        <rdfs:label xml:lang="en">Authority</rdfs:label>
	<rdfs:label xml:lang="es">Autoridad</rdfs:label>
    </owl:Class>
    
    <!-- http://w3id.org/transmodel/organisations#ContactDetails -->

    <owl:Class rdf:about="http://w3id.org/transmodel/organisations#ContactDetails">
        <rdfs:subClassOf rdf:resource="http://schema.org/ContactPoint"/>
        <rdfs:comment xml:lang="en">Contact Details for an Organisation. A subclass of schema:ContactPoint. As such, it can be the domain of properties like schema:url, schema:telephone, schema:email, etc.</rdfs:comment>
	<rdfs:comment xml:lang="es">Información de contacto de una organización. Una subclase de schema:ContactPoint. Como tal, puede ser el dominio de propiedades como schema:url, schema:telephone, schema:email, etc.</rdfs:comment>
        <rdfs:label xml:lang="en">Contact Details</rdfs:label>
	<rdfs:label xml:lang="en">Información de Contacto</rdfs:label>
    </owl:Class>

    <!-- http://w3id.org/transmodel/organisations#Operator -->

    <owl:Class rdf:about="http://w3id.org/transmodel/organisations#Operator">
        <rdfs:subClassOf rdf:resource="http://w3id.org/transmodel/organisations#Organisation"/>
        <owl:disjointWith rdf:resource="http://w3id.org/transmodel/organisations#Authority"/>
        <rdfs:comment xml:lang="en">A company providing Public Transport Services. In GTFS, this is represented as a TransitAgency</rdfs:comment>
	<rdfs:comment xml:lang="es">Una empresa que ofrece servicio de transporte público. En GTFS se representa como una TransitAgency.</rdfs:comment>
        <rdfs:label xml:lang="en">Operator</rdfs:label>
	<rdfs:label xml:lang="es">Operador</rdfs:label>
    </owl:Class>

    <!-- http://w3id.org/transmodel/organisations#Organisation -->

    <owl:Class rdf:about="http://w3id.org/transmodel/organisations#Organisation">
      <rdfs:subClassOf rdf:resource="http://www.w3.org/ns/org#Organization"/>
      <owl:equivalentClass rdf:resource="http://www.w3.org/ns/org#Organization"/>
      <rdfs:comment xml:lang="en">A legally incorporated body associated with any aspect of the transport system</rdfs:comment>
      <rdfs:comment xml:lang="es">Una figura legal asociada con cualquier aspecto del sistema de transporte.</rdfs:comment>
      <rdfs:label xml:lang="en">Organisation</rdfs:label>
      <rdfs:label xml:lang="es">Organización</rdfs:label>
    </owl:Class>

    <!-- http://www.opengis.net/ont/geosparql#Feature -->

    <owl:Class rdf:about="http://www.opengis.net/ont/geosparql#Feature">
        <rdfs:subClassOf rdf:resource="http://www.opengis.net/ont/geosparql#SpatialObject"/>
        <rdfs:comment xml:lang="en">This class represents the top-level feature type. This class is equivalent to GFI_Feature defined in ISO 19156, and it is superclass of all feature types.</rdfs:comment>
	<rdfs:comment xml:lang="es">Esta clase representa una característica de alto nivel, equivalente a GFI_Feature definida en ISP 19156 y es una supercale para todos los tipos de características espaciales.</rdfs:comment>
        <rdfs:isDefinedBy rdf:resource="http://www.opengis.net/spec/geosparql"/>
        <rdfs:label xml:lang="en">Feature</rdfs:label>
	<rdfs:label xml:lang="es">Característica geográfica</rdfs:label>
    </owl:Class>
    

    <!-- http://www.opengis.net/ont/geosparql#Geometry -->

    <owl:Class rdf:about="http://www.opengis.net/ont/geosparql#Geometry">
        <rdfs:subClassOf rdf:resource="http://www.opengis.net/ont/geosparql#SpatialObject"/>
        <rdfs:comment xml:lang="es">Esta clase representa el tipo de geometría de alto nivel. Es equivalente a GFI_Geometry definida en ISO 19156 y es superclase de todos los tipos geométricos.</rdfs:comment>
        <rdfs:comment xml:lang="en">This class represents the top-level geometry type. This class is equivalent to GFI_Geometry defined in ISO 19156, and it is superclass of all geometry types.</rdfs:comment>
        <rdfs:isDefinedBy rdf:resource="http://www.opengis.net/spec/geosparql"/>
        <rdfs:label xml:lang="en">Geometry</rdfs:label>
        <rdfs:label xml:lang="es">Geometría</rdfs:label>
    </owl:Class>
    
   
        <!-- http://www.opengis.net/ont/sf#Point -->

    <owl:Class rdf:about="http://www.opengis.net/ont/sf#Point">
        <rdfs:subClassOf rdf:resource="http://www.opengis.net/ont/geosparql#Geometry"/>
        <rdfs:comment xml:lang="en">This class represents the top-level point type. This 	class is equivalent to GFI_Point defined in ISO 19156, and it is superclass of all point types.</rdfs:comment>
	<rdfs:comment xml:lang="es">Se representa un tipo de punto de alto nivel. Esta clase es equivalente a GFI_Point definida en ISO 19156 y es superclase de todos los tipos de puntos.</rdfs:comment>
        <rdfs:isDefinedBy rdf:resource="http://www.opengis.net/ont/geosparql#"/>
        <rdfs:label xml:lang="en">Geographic Point</rdfs:label>
	<rdfs:label xml:lang="es">Punto geográfico</rdfs:label>
    </owl:Class>

    <!-- http://www.opengis.net/ont/geosparql#SpatialObject -->

    <owl:Class rdf:about="http://www.opengis.net/ont/geosparql#SpatialObject">
      <rdfs:comment xml:lang="en">This class represents the top-level spatial object type. This class is equivalent to GFI_SpatialObject defined in ISO 19156, and it is superclass of all spatial object types.</rdfs:comment>
      <rdfs:comment xml:lang="es">Esta clase representa un tipo de objeto espacial de alto nivel. Es equivalente a GFI SpatialObject difinido en ISO 19156 y es una superclase de todos los tipos de objetos espaciales.</rdfs:comment>
        <rdfs:isDefinedBy rdf:resource="http://www.opengis.net/spec/geosparql"/>
        <rdfs:label xml:lang="en">Spatial Object</rdfs:label>
	<rdfs:label xml:lang="es">Objeto Espacial</rdfs:label>
    </owl:Class>
     
    <!-- http://www.w3.org/2004/02/skos/core#Concept -->

    <owl:Class rdf:about="http://www.w3.org/2004/02/skos/core#Concept">
        <owl:disjointWith rdf:resource="http://www.w3.org/2004/02/skos/core#ConceptScheme"/>
        <dct:issued>2004-02-xx</dct:issued>
        <rdfs:isDefinedBy rdf:resource="http://www.w3.org/2004/02/skos/core#"/>
        <rdfs:label xml:lang="en">Concept</rdfs:label>
	<rdfs:label xml:lang="es">Concepto</rdfs:label>
        <skos:definition xml:lang="en">An abstract idea or notion; a unit of thought.</skos:definition>
	<skos:definition xml:lang="es">Una idea o noción abstracta; una unidad de pensamiento.</skos:definition>
    </owl:Class>


    <!-- http://www.w3.org/2004/02/skos/core#ConceptScheme -->

    <owl:Class rdf:about="http://www.w3.org/2004/02/skos/core#ConceptScheme">
        <dct:issued>2004-02-xx</dct:issued>
        <rdfs:comment xml:lang="en">A concept scheme may be defined to include concepts from different sources.</rdfs:comment>
        <rdfs:comment xml:lang="en">Thesauri, classification schemes, subject heading lists, taxonomies, &apos;folksonomies&apos;, and other types of controlled vocabulary are all examples of concept schemes.  Concept schemes are also embedded in glossaries and terminologies.</rdfs:comment>
	<rdfs:comment xml:lang="es">Un esquema de conceptos definido para incluir conceptos de distintas fuentes.</rdfs:comment>
        <rdfs:isDefinedBy rdf:resource="http://www.w3.org/2004/02/skos/core#"/>
        <rdfs:label xml:lang="en">Concept Scheme</rdfs:label>
	<rdfs:label xml:lang="es">Esquema de conceptos</rdfs:label>
        <skos:definition xml:lang="en">A set of concepts, optionally including statements about semantic relationships between those concepts.</skos:definition>
    </owl:Class>
    
    <!-- http://schema.org/ContactPoint -->

    <owl:Class rdf:about="http://schema.org/ContactPoint">
      <rdfs:label xml:lang="en">Contact Point</rdfs:label>
      <rdfs:label xml:lang="es">Punto de Información de Contacto</rdfs:label>
      <rdfs:comment xml:lang="en">A contact point—for example, Contact section in a website of a Public Transport Organisation Network.</rdfs:comment>
      <rdfs:comment xml:lang="es">Un Punto de Información, por ejemplo, la sección de Contacto en la web de la entidad que participa de alguna manera en el Transporte Público de Autobuses.</rdfs:comment>
    </owl:Class>

    <!--  http://vocab.linkeddata.es/datosabiertos/def/urbanismo-infraestructuras/direccion-postal#DireccionPostal -->

    <owl:Class rdf:about="http://vocab.linkeddata.es/datosabiertos/def/urbanismo-infraestructuras/direccion-postal#DireccionPostal">
      <rdfs:label xml:lang="en">Postal Address</rdfs:label>
      <rdfs:label xml:lang="es">Dirección postal</rdfs:label>
      <rdfs:comment xml:lang="en">A postal address according to the esdir vocabulary.</rdfs:comment>
      <rdfs:comment xml:lang="es">Una dirección postal según el vocabulario esdir.</rdfs:comment>
    </owl:Class>

        <!-- http://vocab.ciudadesabiertas.es/def/transporte/trafico#Incidencia -->

    <owl:Class rdf:about="http://vocab.ciudadesabiertas.es/def/transporte/trafico#Incidencia">
      <rdfs:subClassOf rdf:resource="http://www.opengis.net/ont/geosparql#Feature"/>
      <owl:disjointWith rdf:resource="http://vocab.ciudadesabiertas.es/def/transporte/trafico#Parada"/>
      <rdfs:comment xml:lang="en">Incidence in the traffic system of a city</rdfs:comment>
      <rdfs:comment xml:lang="es">Incidencia que ocurre en el sistema de tráfico de una ciudad</rdfs:comment>
      <rdfs:isDefinedBy rdf:resource="http://vocab.ciudadesabiertas.es/def/transporte/trafico"/>
      <rdfs:label xml:lang="en">Incidence</rdfs:label>
      <rdfs:label xml:lang="es">Incidencia</rdfs:label>
    </owl:Class>

    <!-- http://vocab.ciudadesabiertas.es/def/transporte/trafico#IncidenciaPlanificada -->

    <owl:Class rdf:about="http://vocab.ciudadesabiertas.es/def/transporte/trafico#IncidenciaPlanificada">
        <rdfs:subClassOf rdf:resource="http://vocab.ciudadesabiertas.es/def/transporte/trafico#Incidencia"/>
        <rdfs:comment xml:lang="es">Incidencia planificada, puede ser recurrente o no</rdfs:comment>
        <rdfs:comment xml:lang="en">Planned traffic incidence</rdfs:comment>
        <rdfs:isDefinedBy rdf:resource="http://vocab.ciudadesabiertas.es/def/transporte/trafico"/>
        <rdfs:label xml:lang="es">Incidencia planificada</rdfs:label>
        <rdfs:label xml:lang="en">Planned incidence</rdfs:label>
    </owl:Class>

    <!-- http://www.w3.org/ns/sosa/FeatureOfInterest -->

    <owl:Class rdf:about="http://www.w3.org/ns/sosa/FeatureOfInterest">
      <rdfs:label xml:lang="en">Feature Of Interest</rdfs:label>
      <skos:definition xml:lang="en">The thing whose property is being estimated or calculated in the course of an Observation to arrive at a Result or whose property is being manipulated by an Actuator, or which is being sampled or transformed in an act of Sampling.</skos:definition>
      <rdfs:comment xml:lang="en">The thing whose property is being estimated or calculated in the course of an Observation to arrive at a Result or whose property is being manipulated by an Actuator, or which is being sampled or transformed in an act of Sampling.</rdfs:comment>
      <skos:example xml:lang="en">When measuring the height of a tree, the height is the observed ObservableProperty, 20m may be the Result of the Observation, and the tree is the FeatureOfInterest. A window is a FeatureOfInterest for an automatic window control Actuator.</skos:example>
      <rdfs:isDefinedBy rdf:resource="http://www.w3.org/ns/sosa/"/>
    </owl:Class>

    <!-- http://www.w3.org/ns/sosa/ObservableProperty -->

    <owl:Class rdf:about="http://www.w3.org/ns/sosa/ObservableProperty">
      <rdfs:label xml:lang="en">Observable Property</rdfs:label>
      <skos:definition xml:lang="en">An observable quality (property, characteristic) of a FeatureOfInterest.</skos:definition>
      <rdfs:comment xml:lang="en">An observable quality (property, characteristic) of a FeatureOfInterest.</rdfs:comment>
      <skos:example xml:lang="en">The height of a tree, the depth of a water body, or the temperature of a surface are examples of observable properties, while the value of a classic car is not (directly) observable but asserted.</skos:example>
      <rdfs:isDefinedBy rdf:resource="http://www.w3.org/ns/sosa/"/>
    </owl:Class>

    <!-- http://www.w3.org/ns/sosa/Observation -->

    <owl:Class rdf:about="http://www.w3.org/ns/sosa/Observation">
      <rdfs:label xml:lang="en">Observation</rdfs:label>
      <skos:definition xml:lang="en">Act of carrying out an (Observation) Procedure to estimate or calculate a value of a property of a FeatureOfInterest. Links to a Sensor to describe what made the Observation and how; links to an ObservableProperty to describe what the result is an estimate of, and to a FeatureOfInterest to detail what that property was associated with.</skos:definition>
      <rdfs:comment xml:lang="en">Act of carrying out an (Observation) Procedure to estimate or calculate a value of a property of a FeatureOfInterest. Links to a Sensor to describe what made the Observation and how; links to an ObservableProperty to describe what the result is an estimate of, and to a FeatureOfInterest to detail what that property was associated with</rdfs:comment>
      <skos:example xml:lang="en">The activity of estimating the intensity of an Earthquake using the Mercalli intensity scale is an Observation as is measuring the moment magnitude, i.e., the energy released by said earthquake.</skos:example>
      <rdfs:isDefinedBy rdf:resource="http://www.w3.org/ns/sosa/"/>
    </owl:Class>

    <!-- http://www.w3.org/ns/sosa/Sensor -->

        <owl:Class rdf:about="http://www.w3.org/ns/sosa/Sensor">
      <rdfs:label xml:lang="en">Sensor</rdfs:label>
      <skos:definition xml:lang="en">Device, agent (including humans), or software (simulation) involved in, or implementing, a Procedure. Sensors respond to a stimulus, e.g., a change in the environment, or input data composed from the results of prior Observations, and generate a Result. Sensors can be hosted by Platforms.</skos:definition>
      <rdfs:comment xml:lang="en">Device, agent (including humans), or software (simulation) involved in, or implementing, a Procedure. Sensors respond to a stimulus, e.g., a change in the environment, or input data composed from the results of prior Observations, and generate a Result. Sensors can be hosted by Platforms.</rdfs:comment>
      <skos:example xml:lang="en">Accelerometers, gyroscopes, barometers, magnetometers, and so forth are Sensors that are typically mounted on a modern smart phone (which acts as Platform). Other examples of sensors include the human eyes.</skos:example>
      <rdfs:isDefinedBy rdf:resource="http://www.w3.org/ns/sosa/"/>
    </owl:Class>
    
    <!-- 
	 ///////////////////////////////////////////////////////////////////////////////////////
	 //
	 // Individuals
	 //
	 ///////////////////////////////////////////////////////////////////////////////////////
    -->


    <!-- http://vocab.linkeddata.es/datosabiertos/kos/transporte/trafico/tipo-incidencia -->

    <owl:NamedIndividual rdf:about="http://vocab.linkeddata.es/datosabiertos/kos/transporte/trafico/tipo-incidencia">
	<rdf:type rdf:resource="http://www.w3.org/2004/02/skos/core#ConceptScheme"/>
	<rdfs:label xml:lang="es">tipo de incidencia</rdfs:label>
	<rdfs:label xml:lang="en">type of incidence</rdfs:label>
    </owl:NamedIndividual>

    <!-- http://w3id.org/transmodel/kos/journeys/day-type -->

    <owl:NamedIndividual rdf:about="http://w3id.org/transmodel/kos/journeys/day-type">
        <rdf:type rdf:resource="http://www.w3.org/2004/02/skos/core#ConceptScheme"/>
        <rdfs:comment xml:lang="en">Concept scheme where all the codelists for the types of datatype properties that are included in the Transmodel ontology</rdfs:comment>
        <rdfs:comment xml:lang="en">TODO: determine whether there may be split into serveral kos or not</rdfs:comment>
        <rdfs:label xml:lang="en">day type</rdfs:label>
    </owl:NamedIndividual>
    
    <!-- http://w3id.org/transmodel/kos/journeys/direction-type  -->

    <owl:NamedIndividual rdf:about="http://w3id.org/transmodel/kos/journeys/direction-type/">
	<rdf:type rdf:resource="http://www.w3.org/2004/02/skos/core#ConceptScheme"/>
      <rdfs:label xml:lang="es">tipo de dirección</rdfs:label>
      <rdfs:label xml:lang="en">type of direction</rdfs:label>
      <rdfs:comment xml:lang="es">Tipo de dirección que toma un Viaje de un Vehículo: de entrada, de salida, en el sentido de las agujas del reloj, en el sentido contrario a las agujas del reloj.</rdfs:comment>
      <rdfs:comment xml:lang="en">Type of direction of a Vehicle Journey: inbound, outbound, clockwise or anticlockwise.</rdfs:comment>
    </owl:NamedIndividual>
    
    <!-- http://w3id.org/transmodel/kos/journeys/stop-use-type -->

    <owl:NamedIndividual rdf:about="http://w3id.org/transmodel/kos/journeys/stop-use-type/">
	<rdf:type rdf:resource="http://www.w3.org/2004/02/skos/core#ConceptScheme"/>
      <rdfs:label xml:lang="es">tipo de parada</rdfs:label>
      <rdfs:label xml:lang="en">type of stop</rdfs:label>
      <rdfs:comment xml:lang="es">Tipo de parada en el viaje de un vehículo.</rdfs:comment>
      <rdfs:comment xml:lang="en">Type of stop in a vehicle journey.</rdfs:comment>
    </owl:NamedIndividual>
    
</rdf:RDF>
